Saving state before throwing out a bunch of code in a new branch and moving to explicit substitutions.

coq/Corps/Contexts.v
@@ -13,12 +13,12 @@ Require Import Syntax.
 
 Section Contexts.
   Context {PName : Type} `{EqBool PName}.
-  #[local] Notation mod := (@mod PName).
+  #[local] Abbreviation mod := (@mod PName).
   #[local] Definition ptm := @proc_to_mod PName.
   #[local] Definition PrefixOfT := @PrefixOfT PName.
   Coercion ptm : PName >-> mod.
-  #[local] Notation type := (type PName).
-  #[local] Notation expr := (expr PName).
+  #[local] Abbreviation type := (type PName).
+  #[local] Abbreviation expr := (expr PName).
 
   Record Ctxt :=
     {
@@ -77,6 +77,77 @@ Section Contexts.
     destruct n; [apply base_Prefix | apply locks_bound].
   Qed.
 
+  Definition ctxt_equiv' (Γ Δ : Ctxt) : Prop :=
+    (forall x, snd (vars Γ x) = snd (vars Δ x))
+    /\ (forall x, exists m m', all_locks Γ = mod_app (locks Γ x) m /\ all_locks Δ = mod_app (locks Δ x) m'
+                  /\ mod_app (fst (vars Γ x)) m = mod_app (fst  (vars Δ x)) m')
+    /\ all_locks Γ = all_locks Δ.
+
+  Lemma ctxt_equiv'_refl (Γ : Ctxt) : ctxt_equiv' Γ Γ.
+  Proof using H.
+    split; [| split]; intros; try reflexivity.
+    destruct (prefix_remove_Some (locks Γ x) (all_locks Γ) (locks_bound Γ x)) as [m eq].
+    exists m; exists m; split; [| split].
+    1,2: symmetry; apply readd_remove_prefix with (m2 := all_locks Γ); exact eq.
+    reflexivity.
+  Qed.
+
+  Theorem add_lock_ext' : forall (Γ Δ : Ctxt) m, ctxt_equiv' Γ Δ -> ctxt_equiv' (add_lock Γ m) (add_lock Δ m).
+  Proof using.
+    intros Γ Δ m eqv; destruct eqv as [vars_eq [locks_eq all_locks_eq]]; split; [| split]; cbn;
+      auto.
+    2: rewrite all_locks_eq; reflexivity.
+    intro x; destruct (locks_eq x) as [m1 [m2 [m1_eq [m2_eq locks_eq']]]].
+    exists m1; exists m2; split; [| split].
+    rewrite m1_eq. 2: rewrite m2_eq. 1,2: rewrite mod_app_assoc; reflexivity.
+    exact locks_eq'.
+  Qed.
+
+  Theorem add_var_ext' : forall (Γ Δ : Ctxt) m τ, ctxt_equiv' Γ Δ -> ctxt_equiv' (add_var Γ m τ) (add_var Δ m τ).
+  Proof using.
+    intros Γ Δ m τ [vars_eq [locks_eq al_eq]]; split; [| split]; cbn.
+    - intro x; destruct x; auto.
+    - intro x; destruct x; auto.
+      exists (all_locks Γ); exists (all_locks Δ); split; [symmetry; apply mod_base_app| split; [symmetry; apply mod_base_app|]].
+      cbn. rewrite al_eq. reflexivity.
+    - exact al_eq.
+  Qed.
+
+  #[global] Instance CtxtEquiv'Refl : Reflexive ctxt_equiv' := ctxt_equiv'_refl.
+
+  Lemma ctxt_equiv'_sym : forall Γ Δ, ctxt_equiv' Γ Δ -> ctxt_equiv' Δ Γ.
+  Proof using H.
+    intros Γ Δ [typ_eqv [locks_eqv al_eqv]]; split; [| split]; try intro x; try (symmetry; auto; fail).
+    destruct (locks_eqv x) as [m [m' [eq_m_Γ [eq_m'_Δ vars_eq]]]].
+    exists m'; exists m; auto.
+  Qed.
+
+  #[global] Instance CtxtEquiv'Sym : Symmetric ctxt_equiv' := ctxt_equiv'_sym.
+
+  Lemma mod_app_inj2 : forall (m m1 m2 : mod) , mod_app m m1 = mod_app m m2 -> m1 = m2.
+  Proof using H.
+    intros m m1; revert m; induction m1 as [| m1 IHm1 p]; cbn; intros m m2 eq.
+    - symmetry; apply mod_app_id_inv with (m1 := m); exact eq.
+    - destruct m2 as [|m2 q].
+      -- cbn in eq.
+         assert (mod_size (cons (mod_app m m1) p) = mod_size m) as eq' by (rewrite eq; reflexivity).
+         cbn in eq'; rewrite mod_app_size in eq'; lia.
+      -- cbn in eq; inversion eq; subst; apply IHm1 in H1; rewrite H1; reflexivity.
+  Qed.
+    
+  
+  Lemma ctxt_equiv'_trans : forall Γ Δ E : Ctxt, ctxt_equiv' Γ Δ -> ctxt_equiv' Δ E -> ctxt_equiv' Γ E.
+  Proof using H.
+    intros Γ Δ E [typ_eqv1 [locks_eqv1 al_eqv1]] [typ_eqv2 [locks_eqv2 al_eqv2]];
+      split; [intro x; etransitivity; eauto| split; [| etransitivity; eauto ]].
+    intro x; destruct (locks_eqv1 x) as [m1 [m2 [m1_eq [m2_eq vars_eq1]]]];
+      destruct (locks_eqv2 x) as [m2' [m3 [m2'_eq [m3_eq vars_eq2]]]].
+    assert (m2' = m2) as Heq by (apply mod_app_inj2 with (m := locks Δ x); transitivity (all_locks Δ); auto); subst.
+    exists m1; exists m3; split; [| split]; auto. transitivity (mod_app (fst (vars Δ x)) m2); auto.
+  Qed.
+    
+  #[global] Instance CtxtEquiv'Trans : Transitive ctxt_equiv' := ctxt_equiv'_trans.
+
   Definition ctxt_equiv (Γ Δ : Ctxt) : Prop :=
     (forall x, vars Γ x = vars Δ x)
     /\ (forall x, locks Γ x = locks Δ x)
@@ -112,6 +183,32 @@ Section Contexts.
       Equivalence_Transitive := CtxtEquivTrans;
     |}.
 
+  Theorem add_lock_ext : forall (Γ Δ : Ctxt) m, ctxt_equiv Γ Δ -> ctxt_equiv (add_lock Γ m) (add_lock Δ m).
+  Proof using.
+    intros Γ Δ m eqv; destruct eqv as [vars_eq [locks_eq all_locks_eq]]; split; [| split]; cbn;
+      auto.
+    - intros x; destruct x; cbn; auto.
+      all: rewrite locks_eq; reflexivity.
+    - rewrite all_locks_eq; reflexivity.
+  Qed.
+
+  Theorem add_var_ext : forall (Γ Δ : Ctxt) m τ, ctxt_equiv Γ Δ -> ctxt_equiv (add_var Γ m τ) (add_var Δ m τ).
+  Proof using.
+    intros Γ Δ m τ [vars_eq [locks_eq all_locks_eq]]; split; [| split]; cbn.
+    1,2 : intro x; destruct x.
+    all: auto.
+  Qed.
+
+  Lemma ctxt_equiv_to_equiv' : forall Γ Δ, ctxt_equiv Γ Δ -> ctxt_equiv' Γ Δ.
+  Proof using H PName.
+    intros Γ Δ [vars_eqv [locks_eqv al_eqv]]; split; [| split]; [ intro x; rewrite vars_eqv; reflexivity | | apply al_eqv].
+    intro x. rewrite vars_eqv; rewrite locks_eqv; rewrite al_eqv.
+    destruct (prefix_remove_Some (locks Δ x) (all_locks Δ) (locks_bound Δ x)) as [m eq].
+    exists m; exists m; split; [| split].
+    1,2: symmetry; apply readd_remove_prefix with (m2 := all_locks Δ); exact eq.
+    reflexivity.
+  Qed.
+
   Lemma add_base_lock : forall Γ, ctxt_equiv Γ (add_lock Γ base).
   Proof using.
     intro Γ; split; [|split]; intros; cbn; try rewrite mod_base_app; reflexivity.
@@ -121,31 +218,8 @@ Section Contexts.
   Proof using.
     intros Γ m1 m2; split; [|split]; intros; cbn; try reflexivity; apply mod_app_assoc.
   Qed.
-
-
   
-  Section Lockpointer.
-
-    Record lockpointer (Γ : Ctxt) (m : mod) :=
-      {
-        index : nat;
-        prefix : mod;
-        pred_index : (index = 0 /\ prefix = base) \/ (exists k, index = S k /\ locks Γ k = prefix);
-        at_index : locks Γ index = mod_app prefix m
-      }.
-
-    Lemma before_index : forall (Γ : Ctxt) (m : mod) (ptr : lockpointer Γ m) (n : nat),
-        n < index Γ m ptr ->
-        PrefixOf (locks Γ n) (prefix Γ m ptr).
-    Proof using.
-      intros Γ m ptr n n_lt_index.
-      destruct (pred_index Γ m ptr) as [[eq0 eq_base] | [k [eqS eq_locks]]].
-      - rewrite eq0 in n_lt_index; inversion n_lt_index.
-      - transitivity (locks Γ k).
-        -- apply locks_mono; rewrite eqS in n_lt_index; apply PeanoNat.lt_n_Sm_le; exact n_lt_index.
-        -- rewrite eq_locks; reflexivity.
-    Qed.
-
+  Section ChangeLock.
     
     Program Definition change_lock (Γ : Ctxt) {m1 m2 : mod} (inv : forall n, PrefixOf m1 (locks Γ n) \/ PrefixOf (locks Γ n) m2) :=
       {|
@@ -204,6 +278,12 @@ Section Contexts.
       split; [| split]; try intro x; cbn; auto.
     Qed.
 
+    Lemma change_lock_inv_ext' : forall {Γ : Ctxt} {m1 m2 : mod} (inv1 inv2 : forall n, PrefixOf m1 (locks Γ n) \/ PrefixOf (locks Γ n) m2),
+        ctxt_equiv' (change_lock Γ inv1) (change_lock Γ inv2).
+    Proof using.
+      intros Γ m1 m2 inv1 inv2; apply ctxt_equiv_to_equiv'; apply change_lock_inv_ext.
+    Qed.
+
     Lemma change_lock_ctxt_ext : forall {Γ Δ : Ctxt} {m1 m2 : mod} (inv : forall n, PrefixOf m1 (locks Γ n) \/ PrefixOf (locks Γ n) m2)
                                         (eqv : ctxt_equiv Γ Δ),
         ctxt_equiv (change_lock Γ inv) (change_lock Δ (inv_ext eqv inv)).
@@ -214,6 +294,57 @@ Section Contexts.
       rewrite al_eqv; reflexivity.
     Qed.
 
+
+    Lemma change_prefix_base : forall m1 m2, change_prefix base m1 m2 = Some (mod_app m2 m1).
+    Proof using.
+      intros m1; induction m1; intro m2; cbn; eq_bool; subst.
+      - reflexivity.
+      - inversion eq.
+      - rewrite IHm1. reflexivity.
+    Qed.
+
+    Lemma change_prefix_mod_app : forall m1 m2 m3 m4 m5,
+        change_prefix m1 m2 m3 = Some m4 -> change_prefix m1 (mod_app m2 m5) m3 = Some (mod_app m4 m5).
+    Proof using.
+      intros m1 m2 m3 m4 m5; revert m1 m2 m3 m4; induction m5; intros m1 m2 m3 m4 eq; cbn in *; eq_bool; subst.
+      - exact eq.
+      - exfalso. pose proof (only_prefixes_changable _ _ _ _ eq) as pfx.
+        apply PrefixOf_size in pfx; cbn in pfx; rewrite mod_app_size in pfx; lia.
+      - rewrite IHm5 with (m4 := m4); auto.
+    Qed.
+
+
+
+    
+    (* Lemma change_lock_ctxt_ext' : forall {Γ Δ : Ctxt} {m1 m2 : mod} (inv1 : forall n, PrefixOf m1 (locks Γ n) \/ PrefixOf (locks Γ n) m2) *)
+    (*                                 (inv2 : forall n, PrefixOf m1 (locks Δ n) \/ PrefixOf (locks Δ n) m2) *)
+    (*                                 (eqv : ctxt_equiv' Γ Δ), *)
+    (*     ctxt_equiv' (change_lock Γ inv1) (change_lock Δ inv2). *)
+    (* Proof using. *)
+    (*   intros Γ Δ m1 m2 inv1 inv2 [vars_eqv [locks_eqv al_eqv]]. *)
+    (*   split; [|split]; try intro x; cbn; auto. *)
+    (*   - destruct (locks_eqv x) as [m [m' [m_eq [m'_eq m_prime_eq]]]]. *)
+    (*     destruct (change_prefix m1 (locks Γ x) m2) eqn:eq1; [rewrite m_eq; rewrite (change_prefix_mod_app _ _ _ _ _ eq1)|]; *)
+    (*       destruct (change_prefix m1 (locks Δ x) m2) eqn:eq2. *)
+    (*     -- rewrite m'_eq; rewrite (change_prefix_mod_app _ _ _ _ _ eq2). exists m; exists m'; split; [| split]; auto. *)
+    (*     -- destruct (change_prefix m1 (all_locks Δ) m2) eqn:eq3. *)
+    (*        2: { exists m; exists m'; split; [| split]; auto. } *)
+    (*        pose proof (prefix_changed_to_prefix _ _ _ _ eq3) as pfx. *)
+    (*        destruct (inv2 x) as [pfx' | pfx']; [apply change_prefix_of_prefix with (m3 := m2) in pfx'; apply pfx' in eq2; destruct eq2|]. *)
+    (*        destruct (PrefixOf_peel pfx) as [m3' eq_m3']. *)
+    (*        destruct (PrefixOf_peel pfx') as [m2' eq_m2']. *)
+    (*        rewrite eq_m2' in eq_m3'. rewrite mod_app_assoc in eq_m3'. *)
+    (*        exists m; exists (mod_app m2' m3'); split; [| split]; auto. *)
+           
+
+    (*   change_prefix m1 m2 m3 = Some m4 -> change_prefix m1 (mod_app m2 m5) m3 = Some (mod_app m4 m5) *)
+    (*   destruct (change_prefix m1 (all_locks Γ) m2) eqn:eq2. *)
+    (*   2: { exfalso; apply change_prefix_of_prefix in eq2; auto. rewrite m_eq. transitivity (locks Γ x); auto. apply PrefixOf_app. } *)
+      
+    (*   rewrite m_eq. *)
+      
+    (* Admitted. *)
+
     Lemma change_lock_ext : forall {Γ Δ : Ctxt} {m1 m2 : mod} (inv1 : forall n, PrefixOf m1 (locks Γ n) \/ PrefixOf (locks Γ n) m2)
                               (inv2 : forall n, PrefixOf m1 (locks Δ n) \/ PrefixOf (locks Δ n) m2),
         ctxt_equiv Γ Δ ->
@@ -222,49 +353,543 @@ Section Contexts.
       intros Γ Δ m1 m2 inv1 inv2 eqv;
         transitivity (change_lock Δ (inv_ext eqv inv1)); [apply change_lock_ctxt_ext | apply change_lock_inv_ext].
     Qed.
-    
-    Theorem change_lock_inv_send : forall {Γ : Ctxt} {m : mod} {p : PName} (q : PName) {seen : nat},
-        locks Γ seen = cons m p ->
-        forall n, PrefixOf (cons m p) (locks Γ n)  \/ PrefixOf (locks Γ n) (cons m q).
-    Proof using.
-      intros Γ m p q seen seen_cons n.
-      destruct (PeanoNat.Nat.leb_spec n seen).
-      pose proof (locks_mono Γ H0) as prefix_n_seen; dependent destruction prefix_n_seen.
-      - left; rewrite x; rewrite seen_cons; reflexivity.
-      - rewrite seen_cons in x; inversion x; subst; clear x.
-        right. apply PO_step. exact prefix_n_seen.
-      - left; transitivity (locks Γ seen). rewrite seen_cons; reflexivity.
-        apply locks_mono; apply PeanoNat.Nat.lt_le_incl; exact H0.
-    Qed.           
 
-    Theorem change_lock_inv_up : forall {Γ : Ctxt} {m : mod} (p : PName) {seen : nat},
-        locks Γ seen = m ->
-        forall n, PrefixOf m (locks Γ n) \/ PrefixOf (locks Γ n) (cons m p).
+    Lemma change_locks_prefix_pres : forall {Γ : Ctxt} {m1 m2 : mod} {inv : forall n, PrefixOf m1 (locks Γ n) \/ PrefixOf (locks Γ n) m2}
+                                       (n m : nat),
+        PrefixOf (locks Γ n) (locks Γ m) ->
+        PrefixOf (locks (change_lock Γ inv) n) (locks (change_lock Γ inv) m).
     Proof using.
-      intros Γ m p seen seen_cons n.
-      destruct (PeanoNat.Nat.leb_spec n seen) as [n_le_seen | seen_lt_n].
-      - pose proof (locks_mono Γ n_le_seen) as prefix_n_seen; dependent destruction prefix_n_seen.
-        -- left; rewrite <- seen_cons; rewrite <- x; reflexivity.
-        -- rewrite seen_cons in x; inversion x; subst.
-           right; do 2 apply PO_step; exact prefix_n_seen.
-      - left; transitivity (locks Γ seen). rewrite seen_cons; reflexivity.
-        apply locks_mono; apply PeanoNat.Nat.lt_le_incl; exact seen_lt_n.
+      intros Γ m1 m2 inv n m pfx; cbn.
+      destruct (change_prefix m1 (locks Γ n) m2) eqn:eq1;
+        destruct (change_prefix m1 (locks Γ m) m2) eqn:eq2.
+      - eapply change_prefix_of_prefix'; eauto.
+      - pose proof (only_prefixes_changable _  _ _ _ eq1) as pfx_n.
+        exfalso; apply change_prefix_of_prefix in eq2; auto.
+        transitivity (locks Γ n); auto.
+      - pose proof (only_prefixes_changable _  _ _ _ eq2) as pfx_m.
+        destruct (common_suffix _ _ _ pfx pfx_m). 
+        2: apply change_prefix_of_prefix in eq1; auto; destruct eq1.
+        apply prefix_changed_to_prefix in eq2.
+        transitivity m2; auto.
+        destruct (inv n); auto.
+        apply change_prefix_of_prefix in eq1; auto; destruct eq1.
+      - exact pfx.
     Qed.
 
-    Theorem change_lock_inv_down : forall {Γ : Ctxt} {m : mod} {p : PName} {seen : nat},
-        locks Γ seen = cons m p ->
+    Theorem change_lock_inv_send_all : forall {Γ : Ctxt} {m : mod} {p : PName} (q : PName),
+        PrefixOf (cons m p) (all_locks Γ) ->
+        forall n, PrefixOf (cons m p) (locks Γ n)  \/ PrefixOf (locks Γ n) (cons m q).
+    Proof using.
+      intros Γ m p q pfx n.
+      destruct (common_suffix _ _ _ pfx (locks_bound Γ n)) as [pfx' | pfx']; [left; exact pfx'|].
+      inversion pfx'; subst.
+      left; reflexivity.
+      right; apply PO_step; exact pf.
+    Qed.
+    
+    Theorem change_lock_inv_send : forall {Γ : Ctxt} {m : mod} {p : PName} (q : PName) {seen : nat},
+        PrefixOf (cons m p) (locks Γ seen) ->
+        forall n, PrefixOf (cons m p) (locks Γ n)  \/ PrefixOf (locks Γ n) (cons m q).
+    Proof using.
+      intros Γ m p q seen pfx n.
+      destruct (PeanoNat.Nat.leb_spec n seen).
+      pose proof (locks_mono Γ H0) as prefix_n_seen.
+      destruct (common_suffix _ _ _ pfx prefix_n_seen); auto.
+      inversion H1; subst; [left; reflexivity | right; apply PO_step; auto].
+      left; transitivity (locks Γ seen); [auto | apply locks_mono; apply PeanoNat.Nat.lt_le_incl; auto].
+    Qed.
+
+    Theorem change_lock_inv_up_all : forall {Γ : Ctxt} {m : mod} (p : PName),
+        PrefixOf m (all_locks Γ) ->
+        forall n, PrefixOf m (locks Γ n) \/ PrefixOf (locks Γ n) (cons m p).
+    Proof using.
+      intros Γ m p pfx n.
+      destruct (common_suffix _ _ _ pfx (locks_bound Γ n)) as [pfx' | pfx']; [left; exact pfx'|].
+      right; apply PO_step; exact pfx'.
+    Qed.
+
+    Theorem change_lock_inv_up : forall {Γ : Ctxt} {m : mod} (p : PName) {seen : nat},
+        PrefixOf m (locks Γ seen) ->
+        forall n, PrefixOf m (locks Γ n) \/ PrefixOf (locks Γ n) (cons m p).
+    Proof using.
+      intros Γ m p seen pfx n.
+      destruct (PeanoNat.Nat.leb_spec n seen).
+      pose proof (locks_mono Γ H0) as pfx'.
+      destruct (common_suffix _ _ _ pfx pfx'); auto.
+      right; constructor; auto.
+      left; transitivity (locks Γ seen); [| apply locks_mono; apply PeanoNat.Nat.lt_le_incl]; auto.
+    Qed.
+
+    Theorem change_lock_inv_down_all : forall {Γ : Ctxt} {m : mod} {p : PName},
+        PrefixOf (cons m p) (all_locks Γ) ->
         forall n, PrefixOf (cons m p) (locks Γ n) \/ PrefixOf (locks Γ n) m.
     Proof using.
-      intros Γ m p seen locks_seen n.
-      destruct (PeanoNat.Nat.leb_spec n seen) as [n_le_seen | seen_lt_n].
-      - pose proof (locks_mono Γ n_le_seen) as prefix_n_seen; dependent destruction prefix_n_seen.
-        -- left; rewrite <- locks_seen; rewrite <- x; reflexivity.
-        -- rewrite locks_seen in x; inversion x; subst; clear x.
-           right; auto.
-      - left; transitivity (locks Γ seen). rewrite locks_seen; reflexivity.
-        apply locks_mono; apply PeanoNat.Nat.lt_le_incl; exact seen_lt_n.
-    Qed.    
+      intros Γ m p pfx n.
+      destruct (common_suffix _ _ _ pfx (locks_bound Γ n)) as [pfx' | pfx']; [left; exact pfx'|].
+      inversion pfx'; subst.
+      left; reflexivity.
+      right; exact pf.
+    Qed.
+    
+    Theorem change_lock_inv_down : forall {Γ : Ctxt} {m : mod} {p : PName} {seen : nat},
+        PrefixOf (cons m p) (locks Γ seen) ->
+        forall n, PrefixOf (cons m p) (locks Γ n) \/ PrefixOf (locks Γ n) m.
+    Proof using.
+      intros Γ m p seen pfx n.
+      destruct (PeanoNat.Nat.leb_spec n seen).
+      pose proof (locks_mono Γ H0) as prefix_n_seen.
+      destruct (common_suffix _ _ _ pfx prefix_n_seen); auto.
+      inversion H1; subst; auto; left; reflexivity.
+      left; transitivity (locks Γ seen); [auto | apply locks_mono; apply PeanoNat.Nat.lt_le_incl; auto].
+    Qed.
 
-  End Lockpointer.
+  End ChangeLock.
 
+  Section RemoveLocks.
+
+    Program Definition owner_unqualified (Γ : Ctxt) (x : nat) : mod :=
+      match remove_Prefix (locks Γ x) (all_locks Γ) with
+      | Some m => mod_app (fst (vars Γ x)) m
+      | None => _
+      end.
+    Next Obligation.
+      exfalso; destruct (prefix_remove_Some (locks Γ x) (all_locks Γ) (locks_bound Γ x)) as [m eqm].
+      rewrite eqm in Heq_anonymous; inversion Heq_anonymous.
+    Defined.
+
+    Definition is_owner_unqual (Γ : Ctxt) (x : nat) (m : mod) : Prop :=
+      exists m', mod_app (locks Γ x) m' = all_locks Γ /\
+              m = mod_app (fst (vars Γ x)) m'.
+
+    (* This is easily seen to be true, but Coq can't recognize it because of stupidity. *)
+    Axiom owner_unqualified_spec : forall Γ x m,
+        is_owner_unqual Γ x m <-> owner_unqualified Γ x = m.
+
+    Program Definition remove_locks (Γ : Ctxt) : Ctxt :=
+      {|
+        vars n := (owner_unqualified Γ n, snd (vars Γ n));
+        locks n := base;
+        all_locks := base
+      |}.
+    Next Obligation.
+      reflexivity.
+    Defined.
+    Next Obligation.
+      reflexivity.
+    Defined.
+
+    Lemma remove_locks_equiv' : forall (Γ : Ctxt),
+        ctxt_equiv' Γ (add_lock (remove_locks Γ) (all_locks Γ)).
+    Proof using.
+      intro Γ; split; [intro x; reflexivity | split; [| reflexivity]]; cbn.
+      intro x.
+      destruct (prefix_remove_Some (locks Γ x) (all_locks Γ) (locks_bound Γ x)) as [m eqm].
+      exists m; exists base; split; [| split; [cbn; reflexivity|]].
+      - symmetry; apply readd_remove_prefix; exact eqm.
+      - assert (is_owner_unqual Γ x (mod_app (fst (vars Γ x)) m)) as ou by (exists m; split; auto; apply readd_remove_prefix; exact eqm).
+        rewrite owner_unqualified_spec in ou. rewrite ou.
+        rewrite mod_app_base. reflexivity.
+    Qed.
+      
+  End RemoveLocks.
+
+  Section LockChanging.
+    Definition ctxt_ren (Γ : Ctxt) (ξ : renaming) (mono : forall n m, n <= m -> PrefixOf (locks Γ (ξ n)) (locks Γ (ξ m))): Ctxt :=
+      {|
+        vars n := vars Γ (ξ n);
+        locks n := locks Γ (ξ n);
+        all_locks := all_locks Γ;
+        locks_mono n m lt := mono n m lt;
+        locks_bound n := locks_bound Γ (ξ n);
+      |}.
+
+    Lemma ctxt_ren_ext : forall Γ ξ mono mono',
+        ctxt_equiv (ctxt_ren Γ ξ mono) (ctxt_ren Γ ξ mono').
+    Proof using.
+      intros Γ ξ mono mono'; split; [| split]; cbn; reflexivity.
+    Qed.
+
+    Lemma renup_mono : forall (ξ : renaming) (Γ : Ctxt) g τ, (forall n m, n <= m -> PrefixOf (locks Γ (ξ n)) (locks Γ (ξ m))) ->
+                                                        forall n m, n <= m -> PrefixOf (locks (add_var Γ g τ) (renup ξ n)) (locks (add_var Γ g τ) (renup ξ m)).
+    Proof using.
+      intros ξ Γ g τ mono n m n_le_m.
+      destruct n; destruct m; cbn.
+      - constructor.
+      - apply PrefixOf_base.
+      - inversion n_le_m.
+      - apply mono; apply le_S_n; exact n_le_m.
+    Qed.
+
+    Lemma lock_ren_mono : forall (ξ : renaming) (Γ : Ctxt) p, (forall n m, n <= m -> PrefixOf (locks Γ (ξ n)) (locks Γ (ξ m))) ->
+                                                     forall n m, n <= m -> PrefixOf (locks (add_lock Γ p) (ξ n)) (locks (add_lock Γ p) (ξ m)).
+    Proof using.
+      intros ξ Γ p mono n m n_le_m.
+      cbn. apply PrefixOf_app_mono; auto.
+    Qed.
+
+    Lemma renup_nochange : forall ξ l, (forall n, n <= l -> ξ n = n) -> forall n, n <= S l -> renup ξ n = n.
+    Proof using.
+      intros ξ l nochange n n_le_Sl; destruct n; cbn; auto.
+      apply le_S_n in n_le_Sl. rewrite nochange. reflexivity. exact n_le_Sl.
+    Qed.
+
+    Lemma renup_nochange' : forall ξ l, (forall n, n < l -> ξ n = n) -> forall n, n < S l -> renup ξ n = n.
+    Proof using.
+      intros ξ l nochange n n_lt_Sl; destruct n; cbn; auto.
+      apply PeanoNat.lt_S_n in n_lt_Sl. rewrite nochange. reflexivity. exact n_lt_Sl.
+    Qed.
+
+    Lemma nolocks_change_mono : forall {Γ : Ctxt} {ξ : renaming},
+        (forall n, locks Γ n = locks Γ (ξ n)) ->
+        forall n m, n <= m -> PrefixOf (locks Γ (ξ n)) (locks Γ (ξ m)).
+    Proof using.
+      intros Γ ξ H0 n m H1; repeat rewrite <- H0; apply locks_mono; exact H1.
+    Qed.
+
+    Lemma mono_mono_locks : forall (Γ : Ctxt) (ξ : renaming),
+        (forall n m, n <= m -> ξ n <= ξ m) -> forall n m, n <= m -> PrefixOf (locks Γ (ξ n)) (locks Γ (ξ m)).
+    Proof using.
+      intros Γ ξ H0 n m H1; apply locks_mono; apply H0; exact H1.
+    Qed.
+
+    Lemma mono_renup : forall ξ, (forall n m, n <= m -> ξ n <= ξ m) -> forall n m, n <= m -> renup ξ n <= renup ξ m.
+    Proof using.
+      intros ξ mono n m n_le_m.
+      destruct n; cbn; [apply le_0_n|].
+      destruct m; cbn; [inversion n_le_m|].
+      apply le_S_n in n_le_m; apply le_n_S; apply mono; exact n_le_m.
+    Qed.
+
+    Lemma add_mono : forall n x y, x <= y -> x + n <= y + n. Proof using. lia. Qed.
+
+  End LockChanging.
+  
+  Section FiniteContexts.
+      Inductive FiniteCtxt : Type :=
+    | emptyFC : FiniteCtxt
+    | varFC (m : mod) (τ : type) (Δ : FiniteCtxt) : FiniteCtxt
+    | lockFC (m : mod) (Δ : FiniteCtxt) : FiniteCtxt.
+
+    Fixpoint FiniteCtxt_eqb (Γ Δ : FiniteCtxt) : bool :=
+      match Γ, Δ with
+      | emptyFC, emptyFC => true
+      | varFC m1 τ1 Γ', varFC m2 τ2 Δ' => eqb m1 m2 && eqb τ1 τ2 && FiniteCtxt_eqb Γ' Δ'
+      | lockFC m1 Γ', lockFC m2 Δ' => eqb m1 m2 && FiniteCtxt_eqb Γ' Δ'
+      | _, _ => false 
+      end.
+
+    #[global] Program Instance FiniteCtxtEqBool : EqBool FiniteCtxt :=
+      {
+        eqb := FiniteCtxt_eqb;
+      }.
+    Next Obligation.
+      revert y H0; solve_eqb_liebniz x.
+    Defined.
+    Next Obligation.
+      solve_eqb_refl.
+    Defined.
+
+    Fixpoint FiniteCtxtSize (Δ : FiniteCtxt) : nat :=
+      match Δ with
+      | emptyFC => 0
+      | varFC _ _ Δ => S (FiniteCtxtSize Δ)
+      | lockFC _ Δ => FiniteCtxtSize Δ
+      end.
+
+    Fixpoint addFiniteCtxt (Γ : Ctxt) (Δ : FiniteCtxt) : Ctxt :=
+      match Δ with
+      | emptyFC => Γ
+      | varFC m τ Δ => addFiniteCtxt (add_var Γ m τ) Δ
+      | lockFC m Δ => addFiniteCtxt (add_lock Γ m) Δ
+      end.
+
+    Fixpoint vars_of_finite_ctxt (Δ : FiniteCtxt) : list (mod * type) :=
+      match Δ with
+      | emptyFC => nil
+      | varFC m τ Δ => List.app (vars_of_finite_ctxt Δ) (List.cons (m, τ) nil)
+      | lockFC m Δ => vars_of_finite_ctxt Δ
+      end.
+
+    Definition nth_var (Δ : FiniteCtxt) (n : nat) := List.nth_error (vars_of_finite_ctxt Δ) n.
+
+    Lemma vars_of_finite_ctxt_size : forall Δ, FiniteCtxtSize Δ = List.length (vars_of_finite_ctxt Δ).
+    Proof using.
+      intro Δ; induction Δ; cbn; [reflexivity | |]; rewrite IHΔ; [| reflexivity].
+      rewrite length_app; cbn. rewrite PeanoNat.Nat.add_1_r. reflexivity.
+    Qed.
+
+    Lemma nth_var_size1 : forall Δ n, n < FiniteCtxtSize Δ -> exists m τ, nth_var Δ n = Some (m, τ).
+    Proof using.
+      intros Δ n n_lt_size.
+      destruct (nth_var Δ n) as [[m τ]|] eqn:eq; [exists m; exists τ; reflexivity|].
+      apply nth_error_None in eq; rewrite vars_of_finite_ctxt_size in n_lt_size; lia.
+    Qed.
+
+    Lemma nth_var_size2 : forall Δ n, FiniteCtxtSize Δ <= n -> nth_var Δ n = None.
+    Proof using.
+      intros Δ n n_lt_size.
+      destruct (nth_var Δ n) as [pr|] eqn:eq;[|reflexivity].
+      unfold nth_var in eq.
+      assert (nth_error (vars_of_finite_ctxt Δ) n <> None) as neq by (intro eq'; rewrite eq' in eq; inversion eq).
+      apply nth_error_Some in neq. rewrite vars_of_finite_ctxt_size in n_lt_size. lia.
+    Qed.
+
+    Lemma vars_past_finite_ctxt : forall Γ Δ n,
+        FiniteCtxtSize Δ <= n ->
+        vars (addFiniteCtxt Γ Δ) n = vars Γ (n - FiniteCtxtSize Δ).
+    Proof using.
+      intros Γ Δ; revert Γ; induction Δ; intros Γ n size_le_n; cbn in *.
+      - rewrite PeanoNat.Nat.sub_0_r; reflexivity.
+      - specialize (IHΔ (add_var Γ m τ) n ltac:(lia)); rewrite IHΔ.
+        destruct n; [lia|]. rewrite PeanoNat.Nat.sub_succ_l; [|lia]. rewrite PeanoNat.Nat.sub_succ.
+        reflexivity.
+      - rewrite IHΔ; cbn; [reflexivity | exact size_le_n].
+    Qed.        
+
+    Lemma nth_var_add_ctxt : forall Γ Δ n pr,
+        nth_var Δ n = Some pr ->
+        vars (addFiniteCtxt Γ Δ) n = pr.
+    Proof using.
+      intros Γ Δ; revert Γ; induction Δ; intros Γ n pr eq; unfold nth_var in eq; cbn in *.
+      - destruct n; cbn in eq; inversion eq.
+      - assert (n < (length (vars_of_finite_ctxt Δ ++ [(m, τ)]))) as n_lt_length
+            by (apply nth_error_Some; rewrite eq; discriminate).
+        rewrite length_app in n_lt_length; cbn in n_lt_length.
+        rewrite PeanoNat.Nat.add_1_r in n_lt_length.
+        apply PeanoNat.lt_n_Sm_le in n_lt_length.
+        destruct (Compare_dec.le_lt_eq_dec _ _ n_lt_length) as [l|l].
+        -- apply nth_error_app1 with (l' := [(m, τ)]) in l; rewrite eq in l; symmetry in l.
+           apply IHΔ with (Γ := add_var Γ m τ) in l. exact l.
+        -- assert (length (vars_of_finite_ctxt Δ) <= n) as l' by (apply PeanoNat.Nat.eq_le_incl; auto).
+           apply nth_error_app2 with (l' := [(m, τ)]) in l'; rewrite eq in l'; symmetry in l'; subst.
+           rewrite PeanoNat.Nat.sub_diag in l'; cbn in l'; inversion l'; subst.
+           rewrite vars_past_finite_ctxt; rewrite vars_of_finite_ctxt_size; [| reflexivity].
+           rewrite PeanoNat.Nat.sub_diag; reflexivity.
+      - apply IHΔ. unfold nth_var; auto.
+    Qed.
+
+    Lemma vars_in_finite_ctxt : forall Γ Δ n,
+        n < FiniteCtxtSize Δ ->
+        nth_var Δ n = Some (vars (addFiniteCtxt Γ Δ) n).
+    Proof using.
+      intros Γ Δ n H0.
+      destruct (nth_var Δ n) eqn:eq.
+      rewrite nth_var_add_ctxt with (pr := p); auto.
+      unfold nth_var in eq; apply nth_error_None in eq; rewrite vars_of_finite_ctxt_size in H0; lia.
+    Qed.
+
+    Fixpoint FiniteCtxtLocks (Δ : FiniteCtxt) : mod :=
+      match Δ with
+      | emptyFC => base
+      | varFC _ _ Δ => FiniteCtxtLocks Δ
+      | lockFC m Δ => mod_app (FiniteCtxtLocks Δ) m
+      end.
+
+    Fixpoint locks_at_finite_ctxt_vars (Δ : FiniteCtxt) :=
+      match Δ with
+      | emptyFC => nil
+      | varFC _ _ Δ => locks_at_finite_ctxt_vars Δ ++ [FiniteCtxtLocks Δ]
+      | lockFC _ Δ => locks_at_finite_ctxt_vars Δ
+      end.
+
+    Lemma locks_at_finite_ctxt_vars_size : forall Δ, length (locks_at_finite_ctxt_vars Δ) = FiniteCtxtSize Δ.
+    Proof using.
+      intro Δ; induction Δ; cbn; auto; rewrite length_app; cbn; lia.
+    Qed.
+
+    Definition locks_at (Δ : FiniteCtxt) (x : nat) := nth_error (locks_at_finite_ctxt_vars Δ) x.
+
+    Theorem AddFiniteCtxt_AllLocks : forall (Γ : Ctxt) (Δ : FiniteCtxt),
+        all_locks (addFiniteCtxt Γ Δ) = mod_app (FiniteCtxtLocks Δ) (all_locks Γ).
+    Proof using.
+      intros Γ Δ; revert Γ; induction Δ; intro Γ; cbn; try (rewrite IHΔ; cbn); symmetry;
+        [ apply mod_base_app | reflexivity | apply mod_app_assoc].
+    Qed.
+
+    Theorem AddFiniteCtxt_locks1 : forall (Γ : Ctxt) (Δ : FiniteCtxt) (x : nat),
+        (FiniteCtxtSize Δ) <= x ->
+        locks (addFiniteCtxt Γ Δ) x = mod_app (FiniteCtxtLocks Δ) (locks Γ (x - FiniteCtxtSize Δ)).
+    Proof using.
+      intros Γ Δ; revert Γ; induction Δ; intros Γ x size_le_x; cbn in *.
+      - rewrite PeanoNat.Nat.sub_0_r. symmetry; apply mod_base_app.
+      - rewrite IHΔ; [| lia]. f_equal.
+        destruct x; [inversion size_le_x|]; cbn.
+        destruct (FiniteCtxtSize Δ) eqn:eq_size.
+        -- rewrite PeanoNat.Nat.sub_0_r; reflexivity.
+        -- destruct (x - n) eqn:eq_n'. exfalso; lia.
+           assert (x - S n = n0) as eq by lia; rewrite eq; reflexivity.
+      - rewrite IHΔ; [| exact size_le_x].
+        rewrite mod_app_assoc; reflexivity.
+    Qed.
+
+    Theorem AddFiniteCtxt_locks2 : forall (Γ : Ctxt) (Δ : FiniteCtxt) (x : nat),
+        x < FiniteCtxtSize Δ ->
+        Some (locks (addFiniteCtxt Γ Δ) x) = locks_at Δ x.
+    Proof using.
+      intros Γ Δ; revert Γ; induction Δ; intros Γ x x_lt_size; cbn in *.
+      - inversion x_lt_size.
+      - pose proof (PeanoNat.lt_n_Sm_le _ _ x_lt_size) as x_le_size.
+        destruct (Compare_dec.le_lt_eq_dec _ _ x_le_size).
+        -- rewrite IHΔ; auto.
+           unfold locks_at at 2; cbn; rewrite nth_error_app1; [|rewrite locks_at_finite_ctxt_vars_size; auto].
+           unfold locks_at; reflexivity.
+        -- rewrite AddFiniteCtxt_locks1; [| subst; reflexivity].
+           rewrite e at 1; rewrite PeanoNat.Nat.sub_diag. cbn.
+           unfold locks_at; cbn; rewrite nth_error_app2; [|rewrite locks_at_finite_ctxt_vars_size; lia].
+           rewrite e; rewrite locks_at_finite_ctxt_vars_size; rewrite PeanoNat.Nat.sub_diag; cbn.
+           reflexivity.
+      - apply IHΔ; auto.
+    Qed.
+
+    Theorem extend_rename : forall (Γ : Ctxt) (Δ : FiniteCtxt),
+        ctxt_equiv (ctxt_ren (addFiniteCtxt Γ Δ) (fun n => n + FiniteCtxtSize Δ) (mono_mono_locks (addFiniteCtxt Γ Δ)  (fun n => n + FiniteCtxtSize Δ) (add_mono (FiniteCtxtSize Δ))))
+          (add_lock Γ (FiniteCtxtLocks Δ)).
+    Proof using.
+      intros Γ Δ; split; [| split]; try intro x; cbn.
+      - rewrite vars_past_finite_ctxt; [| lia].
+        assert (x + FiniteCtxtSize Δ - FiniteCtxtSize Δ = x) as e by lia; rewrite e; reflexivity.
+      - rewrite (AddFiniteCtxt_locks1 Γ Δ (x + FiniteCtxtSize Δ)); [| lia].
+        assert (x + FiniteCtxtSize Δ - FiniteCtxtSize Δ = x) as e by lia; rewrite e; reflexivity.
+      - apply AddFiniteCtxt_AllLocks.
+    Qed.
+
+    Fixpoint add_end_var (Δ : FiniteCtxt) (m : mod) (τ : type) : FiniteCtxt :=
+      match Δ with
+      | emptyFC => varFC m τ emptyFC
+      | varFC m' τ' Δ => varFC m' τ' (add_end_var Δ m τ)
+      | lockFC m' Δ => lockFC m' (add_end_var Δ m τ)
+      end.
+
+    Theorem add_end_var_eqv : forall (Γ : Ctxt) (Δ : FiniteCtxt) (m : mod) (τ : type),
+        ctxt_equiv (addFiniteCtxt Γ (add_end_var Δ m τ)) (add_var (addFiniteCtxt Γ Δ) m τ).
+    Proof using.
+      intros Γ Δ; revert Γ; induction Δ; intros Γ m' τ'; cbn; try rewrite IHΔ; reflexivity.
+    Qed.
+
+    Lemma add_end_var_size : forall Δ m τ, FiniteCtxtSize (add_end_var Δ m τ) = S (FiniteCtxtSize Δ).
+    Proof using.
+      intro Δ; induction Δ; intros m' τ'; cbn; try rewrite IHΔ; reflexivity.
+    Qed.
+    
+    Fixpoint add_end_lock (Δ : FiniteCtxt) (m : mod) : FiniteCtxt :=
+      match Δ with
+      | emptyFC => lockFC m emptyFC
+      | varFC m' τ Δ => varFC m' τ (add_end_lock Δ m)
+      | lockFC m' Δ => lockFC m' (add_end_lock Δ m)
+      end.
+
+    Theorem add_end_lock_eqv : forall (Γ : Ctxt) (Δ : FiniteCtxt) (m : mod),
+        ctxt_equiv (addFiniteCtxt Γ (add_end_lock Δ m)) (add_lock (addFiniteCtxt Γ Δ) m).
+    Proof using.
+      intros Γ Δ; revert Γ; induction Δ; intros Γ lck; cbn; try rewrite IHΔ; reflexivity.
+    Qed.
+
+    Lemma add_end_lock_size : forall Δ m, FiniteCtxtSize (add_end_lock Δ m) = FiniteCtxtSize Δ.
+    Proof using.
+      intro Δ; induction Δ; intro m'; cbn; try rewrite IHΔ; reflexivity.
+    Qed.
+
+    Fixpoint FiniteChangeLock (Δ : FiniteCtxt) (m1 m2 : mod) : option FiniteCtxt :=
+      match Δ with
+      | emptyFC => Some emptyFC
+      | varFC m τ Δ =>
+          match FiniteChangeLock Δ m1 m2 with
+          | Some Δ => Some (varFC m τ Δ)
+          | None => None
+          end
+      | lockFC m Δ =>
+          match change_prefix m1 m m2 with
+          | Some m' => Some (lockFC m' Δ)
+          | None =>
+              match remove_Prefix m m1, remove_Prefix m m2 with
+              | Some m1', Some m2' =>
+                  match FiniteChangeLock Δ m1' m2' with
+                  | Some Δ => Some (lockFC m Δ)
+                  | None => None
+                  end 
+              | _, _ => None
+              end
+          end
+      end.
+
+    Lemma change_lock_before_finite_ctxt_inv: forall (Γ : Ctxt) (Δ : FiniteCtxt) (m1 m2 m1' m2' : mod)
+                                            (inv : forall n, PrefixOf m1 (locks (addFiniteCtxt Γ Δ) n) \/ PrefixOf (locks (addFiniteCtxt Γ Δ) n) m2),
+        m1 = mod_app (FiniteCtxtLocks Δ) m1' ->
+        m2 = mod_app (FiniteCtxtLocks Δ) m2' ->
+        forall n, PrefixOf m1' (locks Γ n) \/ PrefixOf (locks Γ n) m2'.
+    Proof using.
+      intros Γ Δ m1 m2 m1' m2' inv eq1 eq2 n.
+      destruct (inv (n + FiniteCtxtSize Δ)) as [pfx | pfx]; rewrite AddFiniteCtxt_locks1 in pfx; try lia; rewrite PeanoNat.Nat.add_sub in pfx.
+      - left. rewrite eq1 in pfx. apply mod_app_prefix with (m1 := FiniteCtxtLocks Δ); exact pfx.
+      - right. rewrite eq2 in pfx. apply mod_app_prefix with (m1 := FiniteCtxtLocks Δ); exact pfx.
+    Qed.
+
+    Lemma FiniteCtxtLocks_LocksAt : forall (Δ : FiniteCtxt) (m : mod) (x : nat),
+        locks_at Δ x = Some m ->
+        PrefixOf m (FiniteCtxtLocks Δ).
+    Proof using.
+      intros Δ; induction Δ as [| m' τ Δ IHΔ | m' Δ IHΔ]; intros m x eq; unfold locks_at in eq; cbn in *.
+      - destruct x; cbn in eq; inversion eq.
+      - destruct (Compare_dec.lt_eq_lt_dec (FiniteCtxtSize Δ) x) as [[size_lt_x | size_eq_x] | x_lt_size].
+        -- rewrite nth_error_app2 in eq; [|rewrite locks_at_finite_ctxt_vars_size; lia].
+           destruct (x - length (locks_at_finite_ctxt_vars Δ)) eqn:eq'.
+           rewrite locks_at_finite_ctxt_vars_size in eq'; exfalso; lia.
+           cbn in eq; destruct n; inversion eq.
+        -- rewrite nth_error_app2 in eq; [|rewrite locks_at_finite_ctxt_vars_size; lia].
+           rewrite locks_at_finite_ctxt_vars_size in eq. rewrite size_eq_x in eq. rewrite PeanoNat.Nat.sub_diag in eq. cbn in eq; inversion eq.
+           reflexivity.
+        -- rewrite nth_error_app1 in eq; [| rewrite locks_at_finite_ctxt_vars_size; exact x_lt_size].
+           apply IHΔ with (x := x); unfold locks_at; exact eq.
+      - transitivity (FiniteCtxtLocks Δ). eapply IHΔ; eauto.
+        apply PrefixOf_app.
+    Qed.
+    
+    Lemma change_lock_before_finite_ctxt : forall (Γ : Ctxt) (Δ : FiniteCtxt) (m1 m2 m1' m2' : mod)
+                                                         (inv : forall n, PrefixOf m1 (locks (addFiniteCtxt Γ Δ) n) \/ PrefixOf (locks (addFiniteCtxt Γ Δ) n) m2)
+                                                         (eq1 : m1 = mod_app (FiniteCtxtLocks Δ) m1')
+                                                         (eq2 : m2 = mod_app (FiniteCtxtLocks Δ) m2'),
+        m1' <> base ->
+        ctxt_equiv (change_lock (addFiniteCtxt Γ Δ) inv)
+          (addFiniteCtxt (change_lock Γ (change_lock_before_finite_ctxt_inv Γ Δ m1 m2 m1' m2' inv eq1 eq2)) Δ).
+    Proof using.
+      intros Γ Δ m1 m2 m1' m2' inv eq1 eq2 neq; split; [| split].
+      - intro x. cbn.
+        destruct (Compare_dec.le_lt_dec (FiniteCtxtSize Δ) x) as [size_le_x | x_lt_size].
+        -- repeat (rewrite vars_past_finite_ctxt; [|exact size_le_x]); reflexivity.
+        -- pose proof (vars_in_finite_ctxt Γ Δ x x_lt_size) as H0;
+             pose proof (vars_in_finite_ctxt (change_lock Γ (change_lock_before_finite_ctxt_inv Γ Δ m1 m2 m1' m2' inv eq1 eq2)) Δ x x_lt_size) as H1.
+           rewrite H1 in H0; inversion H0; reflexivity.
+      - intro x.
+        destruct (Compare_dec.le_lt_dec (FiniteCtxtSize Δ) x) as [size_le_x | x_lt_size].
+        -- repeat (rewrite AddFiniteCtxt_locks1; [| exact size_le_x]).
+           cbn.
+           rewrite (change_common_prefix _ (locks (addFiniteCtxt Γ Δ) x) _ _ _ _ _ eq1 (AddFiniteCtxt_locks1 Γ Δ x size_le_x) eq2).
+           destruct (change_prefix m1' (locks Γ (x - FiniteCtxtSize Δ)) m2') eqn:eq.
+           reflexivity.
+           apply AddFiniteCtxt_locks1; auto.
+        -- pose proof (AddFiniteCtxt_locks2 (change_lock Γ (change_lock_before_finite_ctxt_inv Γ Δ m1 m2 m1' m2' inv eq1 eq2)) Δ x x_lt_size) as H0.
+           pose proof (AddFiniteCtxt_locks2 Γ Δ x x_lt_size) as H1.
+           rewrite <- H1 in H0; inversion H0.
+           cbn. rewrite H3.
+           destruct (change_prefix m1 (locks (addFiniteCtxt Γ Δ) x) m2) eqn:eq; [| reflexivity].
+           pose proof (only_prefixes_changable _ _ _ _ eq).
+           assert (PrefixOf (FiniteCtxtLocks Δ) m1) as H4 by (rewrite eq1; apply PrefixOf_app).
+           symmetry in H1; apply FiniteCtxtLocks_LocksAt in H1.
+           assert (PrefixOf (FiniteCtxtLocks Δ) (locks (addFiniteCtxt Γ Δ) x)) as H5 by (etransitivity; eauto).
+           pose proof (PrefixOf_antisym H1 H5) as H6.
+           rewrite H6 in H2. pose proof (PrefixOf_antisym H2 H4) as H7. clear H0 H3; rewrite H7 in eq1.
+           apply mod_app_id_inv in eq1. destruct (neq eq1).
+      - rewrite AddFiniteCtxt_AllLocks.  cbn. rewrite AddFiniteCtxt_AllLocks.
+        rewrite (change_common_prefix _ _ _ _ _ (all_locks Γ) _ eq1 eq_refl eq2).
+        destruct (change_prefix m1' (all_locks Γ) m2') eqn:eq; reflexivity.
+    Qed.
+
+    Lemma change_lock_after_finite_ctxt : forall (Γ : Ctxt) (Δ : FiniteCtxt) (m1 m2 m1' m2' : mod)
+                                                         (inv : forall n, PrefixOf m1 (locks (addFiniteCtxt Γ Δ) n) \/ PrefixOf (locks (addFiniteCtxt Γ Δ) n) m2),
+        PrefixOf m1 (locks
+        ctxt_equiv (change_lock (addFiniteCtxt Γ Δ) inv)
+          (addFiniteCtxt (change_lock Γ (change_lock_before_finite_ctxt_inv Γ Δ m1 m2 m1' m2' inv eq1 eq2)) Δ).
+           
+    End FiniteContexts.
+  
 End Contexts.
