coq/Corps/Types.v
@@ -5,7 +5,8 @@ Require Import Contexts.
 From Stdlib Require Import RelationClasses.
 From Stdlib Require Import Lia.
 From Stdlib Require Import Program.Equality.
-
+(* From Stdlib Require Lists.List. *)
+(* Import List.ListNotations. *)
 
 Section CorpsTypes.
   Context {PName : Type} `{EqBool PName}.
@@ -20,90 +21,92 @@ Section CorpsTypes.
   
   Section TypeSystem.
 
-    Inductive TypedAtLevel : Ctxt -> nat -> expr -> type -> Prop :=
-    | VarTyping {Γ : Ctxt} {l n : nat} {τ : type} (m : mod) (pf1 : vars Γ n = (m, τ)) (pf2 : locks Γ n = m)
-      : TypedAtLevel Γ l (var n) τ
-    | UnitTyping (Γ : Ctxt) (l : nat) : TypedAtLevel Γ l uu UnitT
-    | AtTyping {Γ : Ctxt} {l : nat} {e : expr} {τ : type} (p : PName) (pf : TypedAtLevel (add_lock Γ p) l e τ)
-      : TypedAtLevel Γ l (atE p e) (AtT p τ)
-    | LetTyping {Γ : Ctxt} {l : nat} {e1 e2 : expr} {τ σ : type} {p : PName}
-        (pf1 : TypedAtLevel Γ l e1 (AtT p τ)) (pf2 : TypedAtLevel (add_var Γ p τ) (S l) e2 σ)
-      : TypedAtLevel Γ l (letAt p e1 e2) σ
-    | PairTyping {Γ : Ctxt} {l : nat} {e1 e2 : expr} {τ1 τ2 : type}
-        (pf1 : TypedAtLevel Γ l e1 τ1) (pf2 : TypedAtLevel Γ l e2 τ2)
-      : TypedAtLevel Γ l (pair e1 e2) (TimesT τ1 τ2)
-    | ProjLTyping {Γ : Ctxt} {l : nat} {e : expr} {τ1 τ2 : type}
-        (pf : TypedAtLevel Γ l e (TimesT τ1 τ2))
-      : TypedAtLevel Γ l (pi1 e) τ1
-    | ProjRTyping {Γ : Ctxt} {l : nat} {e : expr} {τ1 τ2 : type}
-        (pf : TypedAtLevel Γ l e (TimesT τ1 τ2))
-      : TypedAtLevel Γ l (pi2 e) τ2
-    | InlTyping {Γ : Ctxt} {l : nat} {e : expr} {τ1 τ2 : type}
-        (pf : TypedAtLevel Γ l e τ1)
-      : TypedAtLevel Γ l (inl e) (PlusT τ1 τ2)
-    | InrTyping {Γ : Ctxt} {l : nat} {e : expr} {τ1 τ2 : type}
-        (pf : TypedAtLevel Γ l e τ2)
-      : TypedAtLevel Γ l (inr e) (PlusT τ1 τ2)
-    | CaseTyping {Γ : Ctxt} {l : nat} {e1 e2 e3 : expr} {τ1 τ2 σ : type}
-        (pf1 : TypedAtLevel Γ l e1 (PlusT τ1 τ2))
-        (pf2 : TypedAtLevel (add_var Γ base τ1) (S l) e2 σ)
-        (pf3 : TypedAtLevel (add_var Γ base τ2) (S l) e3 σ)
-      : TypedAtLevel Γ l (caseE e1 e2 e3) σ
-    | EfqlTyping {Γ : Ctxt} {l : nat} {e : expr}
-        (pf : TypedAtLevel Γ l e VoidT) (τ : type)
-      : TypedAtLevel Γ l (efql e) τ
-    | LamTyping {Γ : Ctxt} {l : nat} {e : expr} {τ1 τ2 : type}
-        (pf : TypedAtLevel (add_var Γ base τ1) (S l) e τ2)
-      : TypedAtLevel Γ l (lam τ1 e) (ArrT τ1 τ2)
-    | AppTyping {Γ : Ctxt} {l : nat} {e1 e2 : expr} {τ1 τ2 : type}
-        (pf1 : TypedAtLevel Γ l e1 (ArrT τ1 τ2))
-        (pf2 : TypedAtLevel Γ l e2 τ1)
-      : TypedAtLevel Γ l (appE e1 e2) τ2
-    | SendTyping {Γ Γ' : Ctxt} {l seen : nat} {m : mod} {p q : PName}  {e : expr} {τ : type}
-        (locks_seen : locks Γ seen = cons m p)
+    Inductive Typed : Ctxt -> expr -> type -> Prop :=
+    | VarTyping {Γ : Ctxt} {n : nat} {τ : type} (m : mod) (pf1 : vars Γ n = (m, τ)) (pf2 : locks Γ n = m)
+      : Typed Γ (var n) τ
+    | UnitTyping (Γ : Ctxt) : Typed Γ uu UnitT
+    | AtTyping {Γ : Ctxt} {e : expr} {τ : type} (p : PName) (pf : Typed (add_lock Γ p) e τ)
+      : Typed Γ (atE p e) (AtT p τ)
+    | LetTyping {Γ : Ctxt} {e1 e2 : expr} {τ σ : type} {p : PName}
+        (pf1 : Typed Γ e1 (AtT p τ)) (pf2 : Typed (add_var Γ p τ) e2 σ)
+      : Typed Γ (letAt p e1 e2) σ
+    | PairTyping {Γ : Ctxt} {e1 e2 : expr} {τ1 τ2 : type}
+        (pf1 : Typed Γ e1 τ1) (pf2 : Typed Γ e2 τ2)
+      : Typed Γ (pair e1 e2) (TimesT τ1 τ2)
+    | ProjLTyping {Γ : Ctxt} {e : expr} {τ1 τ2 : type}
+        (pf : Typed Γ e (TimesT τ1 τ2))
+      : Typed Γ (pi1 e) τ1
+    | ProjRTyping {Γ : Ctxt} {e : expr} {τ1 τ2 : type}
+        (pf : Typed Γ e (TimesT τ1 τ2))
+      : Typed Γ (pi2 e) τ2
+    | InlTyping {Γ : Ctxt} {e : expr} {τ1 τ2 : type}
+        (pf : Typed Γ e τ1)
+      : Typed Γ (inl e) (PlusT τ1 τ2)
+    | InrTyping {Γ : Ctxt} {e : expr} {τ1 τ2 : type}
+        (pf : Typed Γ e τ2)
+      : Typed Γ (inr e) (PlusT τ1 τ2)
+    | CaseTyping {Γ : Ctxt} {e1 e2 e3 : expr} {τ1 τ2 σ : type}
+        (pf1 : Typed Γ e1 (PlusT τ1 τ2))
+        (pf2 : Typed (add_var Γ base τ1) e2 σ)
+        (pf3 : Typed (add_var Γ base τ2) e3 σ)
+      : Typed Γ (caseE e1 e2 e3) σ
+    | EfqlTyping {Γ : Ctxt} {e : expr}
+        (pf : Typed Γ e VoidT) (τ : type)
+      : Typed Γ (efql e) τ
+    | LamTyping {Γ : Ctxt} {e : expr} {τ1 τ2 : type}
+        (pf : Typed (add_var Γ base τ1) e τ2)
+      : Typed Γ (lam τ1 e) (ArrT τ1 τ2)
+    | AppTyping {Γ : Ctxt} {e1 e2 : expr} {τ1 τ2 : type}
+        (pf1 : Typed Γ e1 (ArrT τ1 τ2))
+        (pf2 : Typed Γ e2 τ1)
+      : Typed Γ (appE e1 e2) τ2
+    | SendTyping {Γ Γ' : Ctxt} {seen : nat} {m : mod} {p q : PName} {e : expr} {τ : type}
+        (* (locks_seen : PrefixOf (cons m p) (all_locks Γ)) *)
+        (locks_seen : PrefixOf (cons m p) (locks Γ seen))
         (eqv : ctxt_equiv Γ' (change_lock Γ (change_lock_inv_send q locks_seen)))
-        (pf : TypedAtLevel Γ' l e τ)
+        (pf : Typed Γ' e τ)
         (cs : CanSend (cons m p) (cons m q))
-        (seen_at_level : seen <= l)
-      : TypedAtLevel Γ l (send e seen m p q) τ
-    | UpTyping {Γ Γ' : Ctxt} {l seen : nat} {m : mod} {p : PName} {e : expr} {τ : type}
-        (locks_seen : locks Γ seen = m)
+      : Typed Γ (send e seen m p q) τ
+    | UpTyping {Γ Γ' : Ctxt} {seen : nat} {m : mod} {p : PName} {e : expr} {τ : type}
+        (locks_seen : PrefixOf m (locks Γ seen))
         (eqv : ctxt_equiv Γ' (change_lock Γ (change_lock_inv_up p locks_seen)))
-        (pf : TypedAtLevel Γ' l e τ)
+        (pf : Typed Γ' e τ)
         (cu : CanUp m (cons m p))
-        (seen_at_level : seen <= l)
-      : TypedAtLevel Γ l (up e seen m p) τ
-    | DownTyping {Γ Γ' : Ctxt} {l seen : nat} {m : mod} {p : PName} {e : expr} {τ : type}
-        (locks_seen : locks Γ seen = cons m p)
+      : Typed Γ (up e seen m p) τ
+    | DownTyping {Γ Γ' : Ctxt} {seen : nat} {m : mod} {p : PName} {e : expr} {τ : type}
+        (locks_seen : PrefixOf (cons m p) (locks Γ seen))
         (eqv : ctxt_equiv Γ' (change_lock Γ (change_lock_inv_down locks_seen)))
-        (pf : TypedAtLevel Γ' l e τ)
+        (pf : Typed Γ' e τ)
         (cu : CanDown (cons m p) m)
-        (seen_at_level : seen <= l)
-      : TypedAtLevel Γ l (down e seen m p) τ
+      : Typed Γ (down e seen m p) τ
     .
 
-    Definition Typed Γ e τ := TypedAtLevel Γ 0 e τ.
+    (* Theorem type_ext' : forall {Γ Δ : Ctxt} {e : expr} {τ : type}, *)
+    (*     Typed Γ e τ -> ctxt_equiv' Γ Δ -> Typed Δ e τ. *)
+    (* Proof using. *)
+    (*   intros Γ Δ e τ typd; revert Δ; induction typd; try (rename Δ into Γ'); intros Δ eqv'; *)
+    (*     pose proof (proj1 eqv') as vars_eq; *)
+    (*     pose proof (proj1 (proj2 eqv')) as locks_eq; *)
+    (*     pose proof (proj2 (proj2 eqv')) as all_locks_eq. *)
+    (*   all: try (econstructor; eauto; fail). *)
+    (*   - specialize (vars_eq n). destruct (vars Δ n) eqn:eq; rewrite pf1 in vars_eq; cbn in vars_eq; subst. *)
+    (*     apply VarTyping with (m := m0); auto. *)
+    (*     destruct (locks_eq n) as [m1 [m2 [eq1 [eq2 eq_owner]]]]. *)
+    (*     rewrite pf1 in eq_owner. rewrite eq in eq_owner. cbn in eq_owner. *)
+    (*     rewrite <- all_locks_eq in eq2. rewrite eq1 in eq2. *)
+    (*     rewrite eq2 in eq_owner. apply mod_app_back with (m3 := m2); auto. *)
+    (*   - apply AtTyping; apply IHtypd; apply add_lock_ext'; auto. *)
+    (*   - apply @LetTyping with (τ := τ). apply IHtypd1; auto. apply IHtypd2; auto. apply add_var_ext'; auto. *)
+    (*   - apply @CaseTyping with (τ1 := τ1) (τ2 := τ2). apply IHtypd1; auto. apply IHtypd2. 2: apply IHtypd3. *)
+    (*     all: apply add_var_ext'; auto. *)
+    (*   - apply @LamTyping. apply IHtypd. apply add_var_ext'; auto. *)
+    (*   - pose proof (locks_seen) as locks_seen'; rewrite all_locks_eq in locks_seen'. *)
+    (*     eapply SendTyping with (locks_seen := locks_seen'); auto. reflexivity. apply IHtypd. etransitivity; [exact eqv|]. apply change_lock_ctxt_ext'; auto. *)
 
-    Theorem add_lock_ext : forall (Γ Δ : Ctxt) m, ctxt_equiv Γ Δ -> ctxt_equiv (add_lock Γ m) (add_lock Δ m).
+    Theorem type_ext : forall {Γ Δ : Ctxt} {e : expr} {τ : type},
+        Typed Γ e τ -> (ctxt_equiv Γ Δ) -> Typed Δ e τ.
     Proof using.
-      intros Γ Δ m eqv; destruct eqv as [vars_eq [locks_eq all_locks_eq]]; split; [| split]; cbn;
-        auto.
-      - intros x; destruct x; cbn; auto.
-        all: rewrite locks_eq; reflexivity.
-      - rewrite all_locks_eq; reflexivity.
-    Qed.
-
-    Theorem add_var_ext : forall (Γ Δ : Ctxt) m τ, ctxt_equiv Γ Δ -> ctxt_equiv (add_var Γ m τ) (add_var Δ m τ).
-    Proof using.
-      intros Γ Δ m τ [vars_eq [locks_eq all_locks_eq]]; split; [| split]; cbn.
-      1,2 : intro x; destruct x.
-      all: auto.
-    Qed.
-
-    Theorem type_level_ext : forall (Γ Δ : Ctxt) (l : nat) (e : expr) (τ : type),
-        TypedAtLevel Γ l e τ -> (ctxt_equiv Γ Δ) -> TypedAtLevel Δ l e τ.
-    Proof using.
-      intros Γ Δ l e τ typd; revert Δ; induction typd; try (rename Δ into Γ'); intros Δ' eqv';
+      intros Γ Δ e τ typd; revert Δ; induction typd; try (rename Δ into Γ'); intros Δ' eqv';
         pose proof (proj1 eqv') as vars_eq;
         pose proof (proj1 (proj2 eqv')) as locks_eq;
         pose proof (proj2 (proj2 eqv')) as all_locks_eq;
@@ -118,14 +121,14 @@ Section CorpsTypes.
               | [ _ : locks Δ n = x |- _ ] => fail
               | _ => assert (locks Δ n = x) by (rewrite <- H'; exact H)
               end
-          | [ IH : forall Δ, ctxt_equiv (add_lock ?Γ ?m) Δ -> TypedAtLevel Δ ?l ?e ?τ, H : ctxt_equiv ?Γ ?Δ |- _ ] =>
+          | [ IH : forall Δ, ctxt_equiv (add_lock ?Γ ?m) Δ -> Typed Δ ?e ?τ, H : ctxt_equiv ?Γ ?Δ |- _ ] =>
               lazymatch goal with
-              | [ _ : TypedAtLevel (add_lock Δ m) l e τ |- _ ] => fail
+              | [ _ : Typed (add_lock Δ m) e τ |- _ ] => fail
               | _ => pose proof (IH (add_lock Δ m) (add_lock_ext Γ Δ m H))
               end
-          | [ IH : forall Δ, ctxt_equiv (add_var ?Γ ?m ?τ') Δ -> TypedAtLevel Δ ?level ?e ?τ, H : ctxt_equiv ?Γ ?Δ |- _ ] =>
+          | [ IH : forall Δ, ctxt_equiv (add_var ?Γ ?m ?τ') Δ -> Typed Δ ?e ?τ, H : ctxt_equiv ?Γ ?Δ |- _ ] =>
               lazymatch goal with
-              | [ _ : TypedAtLevel (add_var Δ m τ') level e τ |- _ ] => fail
+              | [ _ : Typed (add_var Δ m τ') e τ |- _ ] => fail
               | _ => pose proof (IH (add_var Δ m τ') (add_var_ext Γ Δ m τ' H))
               end
           (* | [ IH : forall Δ, ctxt_equiv (addFiniteCtxt ?Γ ?E) Δ -> TypedAtLevel Δ ?l ?e ?τ, H : ctxt_equiv ?Γ ?Δ |- _ ] => *)
@@ -135,190 +138,485 @@ Section CorpsTypes.
           (*     end *)
           end;
         try (econstructor; eauto; fail).
-      - apply @SendTyping with (Γ' := Γ') (locks_seen := H0); auto.
+      - eapply @SendTyping with (Γ' := Γ'); eauto. 
         etransitivity; [exact eqv | apply change_lock_ext; auto].
-      - apply @UpTyping with (Γ' := Γ') (locks_seen := H0); auto.
+        Unshelve. rewrite <- locks_eq; auto.
+      - eapply @UpTyping with (Γ' := Γ'); eauto.
         etransitivity; [exact eqv | apply change_lock_ext; auto].
-      - apply @DownTyping with (Γ' := Γ') (locks_seen := H0); auto.
+        Unshelve. rewrite <- locks_eq; auto.
+      - eapply @DownTyping with (Γ' := Γ'); eauto.
         etransitivity; [exact eqv | apply change_lock_ext; auto].
+        Unshelve. rewrite <- locks_eq; auto.
     Qed.
 
-    Theorem type_ext : forall (Γ Δ : Ctxt) (e : expr) (τ : type),
-        Typed Γ e τ -> (ctxt_equiv Γ Δ) -> Typed Δ e τ.
+    Theorem exchange : forall {Γ Δ : Ctxt} {e : expr} {ξ : renaming} {τ : type}
+                        (nolocks_change : forall n, locks Γ n = locks Γ (ξ n)),
+        ctxt_equiv (ctxt_ren Γ ξ (nolocks_change_mono nolocks_change)) Δ ->
+        Typed Δ e τ -> Typed Γ (ren e ξ) τ.
     Proof using.
-      intros Γ Δ e τ H0 H1; eapply type_level_ext; eauto.
-    Qed.
-    
-    Definition ctxt_ren (Γ : Ctxt) (ξ : renaming) (mono : forall n m, n <= m -> PrefixOf (locks Γ (ξ n)) (locks Γ (ξ m))): Ctxt :=
-      {|
-        vars n := vars Γ (ξ n);
-        locks n := locks Γ (ξ n);
-        all_locks := all_locks Γ;
-        locks_mono n m lt := mono n m lt;
-        locks_bound n := locks_bound Γ (ξ n);
-      |}.
-
-    Lemma ctxt_ren_ext : forall Γ ξ mono mono',
-        ctxt_equiv (ctxt_ren Γ ξ mono) (ctxt_ren Γ ξ mono').
-    Proof using.
-      intros Γ ξ mono mono'; split; [| split]; cbn; reflexivity.
-    Qed.
-
-    Lemma renup_mono : forall (ξ : renaming) (Γ : Ctxt) g τ, (forall n m, n <= m -> PrefixOf (locks Γ (ξ n)) (locks Γ (ξ m))) ->
-                                                        forall n m, n <= m -> PrefixOf (locks (add_var Γ g τ) (renup ξ n)) (locks (add_var Γ g τ) (renup ξ m)).
-    Proof using.
-      intros ξ Γ g τ mono n m n_le_m.
-      destruct n; destruct m; cbn.
-      - constructor.
-      - apply PrefixOf_base.
-      - inversion n_le_m.
-      - apply mono; apply le_S_n; exact n_le_m.
-    Qed.
-
-    Lemma lock_ren_mono : forall (ξ : renaming) (Γ : Ctxt) p, (forall n m, n <= m -> PrefixOf (locks Γ (ξ n)) (locks Γ (ξ m))) ->
-                                                     forall n m, n <= m -> PrefixOf (locks (add_lock Γ p) (ξ n)) (locks (add_lock Γ p) (ξ m)).
-    Proof using.
-      intros ξ Γ p mono n m n_le_m.
-      cbn. apply PrefixOf_app_mono; auto.
-    Qed.
-
-    Lemma renup_nochange : forall ξ l, (forall n, n < l -> ξ n = n) -> forall n, n < S l -> renup ξ n = n.
-    Proof using.
-      intros ξ l nochange n n_lt_Sl; destruct n; cbn; auto.
-      apply PeanoNat.lt_S_n in n_lt_Sl. rewrite nochange. reflexivity. exact n_lt_Sl.
-    Qed.
-
-    Lemma nolocks_change_mono : forall {Γ : Ctxt} {ξ : renaming},
-        (forall n, locks Γ n = locks Γ (ξ n)) ->
-        forall n m, n <= m -> PrefixOf (locks Γ (ξ n)) (locks Γ (ξ m)).
-    Proof using.
-      intros Γ ξ H0 n m H1; repeat rewrite <- H0; apply locks_mono; exact H1.
-    Qed.
-
-
-    Lemma weakening_at_level : forall (Γ Δ : Ctxt) (l : nat) (e : expr) (ξ : renaming) (τ : type)
-                                 (locks_no_change : forall n, locks Γ n = locks Γ (ξ n)),
-        ctxt_equiv (ctxt_ren Γ ξ (nolocks_change_mono locks_no_change)) Δ ->
-        (forall n, n < l -> ξ n = n) ->
-        TypedAtLevel Δ l e τ -> TypedAtLevel Γ l (ren e ξ) τ.
-    Proof using.
-      intros Γ Δ l e ξ τ mono eqv ξ_eq typ; revert Γ ξ mono eqv ξ_eq; induction typ; try rename Γ'' into Γ2;
-        intros Γ'' ξ mono ctxt_eqv ξ_eq; cbn.
-      all: pose proof ctxt_eqv as [vars_eqv [locks_eqv al_eqv]].
+      intros Γ Δ e ξ τ nochange eqv typ; revert Γ ξ nochange eqv; induction typ; try rename Γ'' into Γ2;
+        intros Γ'' ξ nochange ctxt_eqv; cbn in *.
+      all: pose proof ctxt_eqv as [vars_eqv [locks_eqv al_eqv]]; cbn in *.
       all: try (econstructor; eauto; fail).
-      - econstructor; eauto.
-        rewrite <- mono.
-        specialize (vars_eqv n); cbn in vars_eqv; rewrite vars_eqv.
-        specialize (locks_eqv n); cbn in locks_eqv; rewrite locks_eqv.
-        rewrite pf1. rewrite pf2. reflexivity.
-      - econstructor; eauto.
-        eapply IHtyp; eauto.
-        split; [| split]; cbn; eauto.
-        2: cbn in al_eqv; rewrite al_eqv; reflexivity.
-        intro x; specialize (locks_eqv x); cbn in locks_eqv; rewrite locks_eqv; reflexivity.
-        Unshelve. cbn; intro n; rewrite <- mono; reflexivity.
-      - econstructor; eauto.
-        eapply IHtyp2. 2: apply renup_nochange; auto. split; [| split]; try intro x; cbn; auto.
-        all: destruct x; cbn; auto. apply vars_eqv. apply locks_eqv.
-        Unshelve. intro n; cbn; destruct n; cbn; [reflexivity | apply mono].
-      - econstructor; eauto.
-        eapply IHtyp2. 3: eapply IHtyp3. all: try eapply renup_nochange; eauto.
-        all: split; [| split]; try intro x; cbn; try reflexivity; try destruct x; cbn; auto.
-        1,3: apply vars_eqv. all: apply locks_eqv.
-        Unshelve. all: intro n; destruct n; cbn; auto.
-      - econstructor; eauto.
-        eapply IHtyp; [|apply renup_nochange; auto].
-        split; [| split]; try intro x; cbn; auto; destruct x; cbn; auto.
-        apply vars_eqv. apply locks_eqv.
-        Unshelve. intro n; destruct n; cbn; auto.
-      - assert (locks Γ'' (ξ seen) = cons m p) as locks_seen'
-            by (specialize (locks_eqv seen); cbn in locks_eqv;
-                rewrite locks_eqv; apply locks_seen).
-        assert (locks Γ'' seen = cons m p) as locks_seen''
-            by (rewrite mono; apply locks_seen').
-        eapply @SendTyping with (Γ' := change_lock Γ'' (change_lock_inv_send q locks_seen'')); eauto;
-          [reflexivity|].
-        eapply IHtyp; auto.
-        destruct eqv as [vars_eqv' [locks_eqv' al_eqv']].
-        split; [| split]; cbn; try intro x.
-        -- specialize (vars_eqv x); cbn in vars_eqv; rewrite vars_eqv.
-           specialize (vars_eqv' x); cbn in vars_eqv'; symmetry; apply vars_eqv'.
-        -- specialize (locks_eqv x); cbn in locks_eqv; rewrite locks_eqv.
-           specialize (locks_eqv' x); cbn in locks_eqv'.
-           symmetry; apply locks_eqv'.
-        -- cbn in al_eqv; rewrite al_eqv; cbn in al_eqv'; symmetry; apply al_eqv'.
-           Unshelve. intro n; cbn; rewrite <- mono; reflexivity.
-      - 
-          
-        
-        
-        
+      - apply VarTyping with (m := m).
+        specialize (vars_eqv n); cbn in vars_eqv; rewrite vars_eqv; auto.
+        specialize (locks_eqv n); cbn in locks_eqv; rewrite locks_eqv; auto.
+      - econstructor; eauto. unshelve eapply IHtyp; cbn. intro n; f_equal; apply nochange.
+        split; [| split]; try intro; cbn; auto; f_equal; auto.
+      - econstructor; eauto. unshelve eapply IHtyp2; cbn.
+        intro n; destruct n; cbn; auto.
+        split; [| split]; try intro x; cbn; auto.
+        all: destruct x; cbn; auto.
+      - econstructor; eauto; [unshelve eapply IHtyp2 | unshelve eapply IHtyp3]; cbn.
+        1,3: intro n; destruct n; cbn; auto.
+        all: split; [| split]; try intro x; cbn; auto.
+        all: destruct x; cbn; auto.
+      - econstructor; eauto. unshelve eapply IHtyp; cbn.
+        intro n; destruct n; cbn; auto.
+        split; [| split]; try intro x; cbn; auto.
+        all: destruct x; cbn; auto.
+      - destruct eqv as [vars_eqv' [locks_eqv' al_eqv']].
+        eapply @SendTyping; eauto. reflexivity. unshelve eapply IHtyp; auto.
+        intro n; cbn; rewrite <- nochange; reflexivity.
+        split; [| split]; try intro x; auto.
+        cbn. rewrite vars_eqv; auto.
+        cbn; rewrite locks_eqv; rewrite locks_eqv'; auto.
+        cbn; rewrite al_eqv; rewrite al_eqv'; auto.
+        Unshelve.  rewrite nochange; rewrite locks_eqv; apply locks_seen.
+      - destruct eqv as [vars_eqv' [locks_eqv' al_eqv']].
+        eapply @UpTyping; eauto. reflexivity. unshelve eapply IHtyp; auto.
+        intro n; cbn; rewrite <- nochange; reflexivity.
+        split; [| split]; try intro x; auto.
+        cbn. rewrite vars_eqv; auto.
+        cbn; rewrite locks_eqv; rewrite locks_eqv'; auto.
+        cbn; rewrite al_eqv; rewrite al_eqv'; auto.
+        Unshelve.  rewrite nochange; rewrite locks_eqv; apply locks_seen.
+      - destruct eqv as [vars_eqv' [locks_eqv' al_eqv']].
+        eapply @DownTyping; eauto. reflexivity. unshelve eapply IHtyp; auto.
+        intro n; cbn; rewrite <- nochange; reflexivity.
+        split; [| split]; try intro x; auto.
+        cbn. rewrite vars_eqv; auto.
+        cbn; rewrite locks_eqv; rewrite locks_eqv'; auto.
+        cbn; rewrite al_eqv; rewrite al_eqv'; auto.
+        Unshelve.  rewrite nochange; rewrite locks_eqv; apply locks_seen.
+    Qed.
 
+    Theorem weakening : forall  {Γ Δ : Ctxt} {e : expr} {ξ : renaming} {τ : type}
+                           (mono : forall n m, n <= m -> ξ n <= ξ m),
+        ctxt_equiv (ctxt_ren Γ ξ (mono_mono_locks Γ ξ  mono)) Δ ->
+        Typed Δ e τ -> Typed Γ (renseen (ren e ξ) ξ) τ.
+    Proof using.
+      intros Γ Δ e ξ τ mono eqv typd; revert Γ ξ mono eqv; induction typd;
+        intros Γ'' ξ mono ctxt_eqv; cbn.
+      all: pose proof ctxt_eqv as [vars_eqv [locks_eqv al_eqv]]; cbn in *.
+      all: try (econstructor; eauto; fail).
+      - econstructor; [rewrite vars_eqv | rewrite locks_eqv]; eauto.
+      - econstructor. apply IHtypd with (mono := mono).
+        split; [| split]; try intro x; cbn; auto; [rewrite locks_eqv | rewrite al_eqv]; auto.
+      - econstructor. apply IHtypd1 with (mono := mono).
+        split; [| split]; try intro x; cbn; auto.
+        apply IHtypd2 with (mono := mono_renup ξ mono). 
+        split; [| split]; try intro x; cbn.
+        3: apply al_eqv.
+        all: destruct x; cbn; auto.
+      - econstructor. apply IHtypd1 with (mono := mono); auto.
+        apply IHtypd2 with (mono := mono_renup ξ mono).
+        2: apply IHtypd3 with (mono := mono_renup ξ mono).
+        all: split; [| split]; try intro x; cbn; auto.
+        all: destruct x; cbn; auto.
+      - econstructor. apply IHtypd with (mono := mono_renup ξ mono).
+        split; [| split]; try intro x; cbn; auto.
+        all: destruct x; cbn; auto.
+      - eapply @SendTyping; [reflexivity | | auto].
+        Unshelve. 2: rewrite locks_eqv; auto.
+        eapply IHtypd.
+        pose proof eqv as [vars_eqv' [locks_eqv' al_eqv']]; cbn in vars_eqv'.
+        split; [| split]; try intro x; cbn.
+        rewrite vars_eqv; symmetry; apply vars_eqv'.
+        rewrite locks_eqv; symmetry; apply locks_eqv'.
+        rewrite al_eqv; symmetry; apply al_eqv'.
+      - eapply @UpTyping; [reflexivity | | auto].
+        Unshelve. 2: auto. 2: rewrite locks_eqv; auto.
+        unshelve eapply IHtypd; auto.
+        pose proof eqv as [vars_eqv' [locks_eqv' al_eqv']]; cbn in vars_eqv'.
+        split; [| split]; try intro x; cbn.
+        rewrite vars_eqv; symmetry; apply vars_eqv'.
+        rewrite locks_eqv; symmetry; apply locks_eqv'.
+        rewrite al_eqv; symmetry; apply al_eqv'.          
+      - eapply @DownTyping; [reflexivity | | auto].
+        Unshelve. 2: auto. 2: rewrite locks_eqv; auto.
+        unshelve eapply IHtypd; auto.
+        pose proof eqv as [vars_eqv' [locks_eqv' al_eqv']]; cbn in vars_eqv'.
+        split; [| split]; try intro x; cbn.
+        rewrite vars_eqv; symmetry; apply vars_eqv'.
+        rewrite locks_eqv; symmetry; apply locks_eqv'.
+        rewrite al_eqv; symmetry; apply al_eqv'.          
+    Qed.        
+        
   End TypeSystem.
 
   Section Substitution.
 
-    Definition TypedSubst (Γ : Ctxt) (σ : substitution) (Δ : Ctxt) :=
-      all_locks Γ = all_locks Δ /\
-      forall x m,
-        mod_app m (locks Γ x) = fst (vars Γ x) -> 
-        Typed (add_lock Δ m) (σ x) (snd (vars Γ x)).
+    Fixpoint add_vars (Γ : Ctxt) (xs : list (mod * type)) :=
+      match xs with
+      | nil => Γ
+      | List.cons (m, τ) xs =>add_var (add_vars Γ xs) m τ
+      end.
 
-    Lemma id_subst_typed: forall Γ, TypedSubst Γ (fun x => var x) Γ.
-    Proof using.
-      intros Γ; split; [reflexivity | intros x m eq].
-      apply VarTyping with (m := fst (vars Γ x)); cbn; auto.
-      apply surjective_pairing.
-    Qed.      
+    Fixpoint finite_substitution (es : list expr) : substitution :=
+      match es with
+      | nil => fun x => var x
+      | List.cons e es => fun x =>
+                   match x with
+                   | 0 => e
+                   | S y => finite_substitution es y
+                   end
+      end.
 
-    Lemma substup_typed : forall Γ Δ σ g τ,
-        TypedSubst Γ σ Δ -> TypedSubst (add_var Γ g τ) (substup σ) (add_var Δ g τ).
+
+    (* Fixpoint typed_finite_substitution (Γ : Ctxt) (Δ : FiniteCtxt) (es : list expr) : Prop := *)
+    (*   match Δ, es with *)
+    (*   | emptyFC, nil => True *)
+    (*   | varFC m τ Δ, List.cons e es => Typed (add_lock Γ m) e τ /\ typed_finite_substitution Γ Δ es *)
+    (*   | lockFC m Δ, es => typed_finite_substitution Γ Δ es *)
+    (*   | _, _ => False *)
+    (*   end. *)
+
+    Fixpoint snoc {A : Type} (xs : list A) (x : A) : list A :=
+      match xs with
+      | List.cons x' xs' => List.cons x' (snoc xs' x)
+      | List.nil => List.cons x nil
+      end.
+
+    Lemma snoc_app: forall {A : Type} (xs : list A) (x : A), snoc xs x = (xs ++ (x :: nil))%list.
     Proof using.
-      intros Γ Δ σ g τ [al_eqv typd]; split; [exact al_eqv|]; intros x m eq.
-      destruct x; cbn in *; subst.
-      - apply VarTyping with (m := g); cbn; reflexivity.
-      - eapply weakening with (Δ := add_lock Δ m).
-        split; [|split]; try (intro y); cbn; auto.
-        apply typd; auto.
-        Unshelve.
-        intros n m0 H0; cbn; apply mod_app_mono_l; apply locks_mono; auto.
+      intros A xs; induction xs as [| x' xs IHxs]; intro x; cbn; [| rewrite IHxs]; reflexivity.
     Qed.
 
-    Theorem subst_typed : forall Γ Δ e σ τ, Typed Γ e τ -> TypedSubst Γ σ Δ -> Typed Δ (subst e σ) τ.
+    Lemma snoc_length : forall {A : Type} (xs : list A) (x : A), length (snoc xs x) = S (length xs).
     Proof using.
-      intros Γ Δ e σ τ typed; revert Δ σ; induction typed; try (rename σ into τ');
-        intros Γ'' σ typeds; cbn;
-        try (econstructor; eauto;
-             repeat lazymatch goal with
-               | [ H : ?P |- ?P ] => exact H
-               | [ IH : forall Δ σ, TypedSubst ?Γ σ Δ -> Typed Δ (subst ?e σ) ?τ, H : TypedSubst ?Γ ?σ ?Δ |- Typed ?Δ (subst ?e ?σ) ?τ ] =>
-                   exact (IH Δ σ H)
-               | [H : TypedSubst ?Γ ?σ ?Δ |- context[add_var ?Δ ?p ?τ] ] =>
-                   lazymatch goal with
-                   | [ _ : TypedSubst (add_var Γ p τ) (substup σ) (add_var Δ p τ) |- _ ] => fail
-                   | _ => 
-                       assert (TypedSubst (add_var Γ p τ) (substup σ) (add_var Δ p τ)) by (exact (substup_typed Γ Δ σ p τ H))
-                   end
-               | [ H : TypedSubst ?Γ ?σ ?Δ |- context[all_locks ?Δ]] =>
-                   lazymatch goal with
-                   | [_ : all_locks Γ = all_locks Δ |- _ ] => fail
-                   | _ => let eq := fresh "eq" in assert (all_locks Γ = all_locks Δ) as eq by (destruct H as [al_eqv _]; exact al_eqv);
-                                                rewrite <- eq
-                   end
-          end; fail).
-      - destruct typeds as [al_eqv typeds].
-        specialize (typeds n base); cbn in typeds.
-        rewrite pf1 in typeds; cbn in typeds.
-        rewrite mod_base_app in typeds; specialize (typeds pf2).
-        apply type_ext with (Γ := add_lock Γ'' base); [exact typeds | symmetry; apply add_base_lock].
-      - apply AtTyping; apply IHtyped.
-        destruct typeds as [al_eqv typeds]; split; [cbn; rewrite al_eqv; reflexivity|].
-        intros x m; cbn; intro eq.
-        apply type_ext with (Γ := add_lock Γ'' (mod_app m p)); [|apply add_two_locks].
-        rewrite <- mod_app_assoc in eq.
-        apply typeds; exact eq.
-    Qed.                                             
+      intros A xs; induction xs as [| y xs IHxs]; intro x; cbn; [| rewrite IHxs]; reflexivity.
+    Qed.
 
+    Inductive typed_finite_substitution : Ctxt -> FiniteCtxt -> list expr -> Prop :=
+    | TypedEmptySubst : forall (Γ : Ctxt), typed_finite_substitution Γ emptyFC nil
+    |  TypedVarCtxt : forall (Γ : Ctxt) (Δ : FiniteCtxt) (m : mod) (τ : type) (e : expr) (es : list expr),
+        Typed (add_lock (add_lock Γ (FiniteCtxtLocks Δ)) m) e τ ->
+        typed_finite_substitution  Γ Δ es ->
+        typed_finite_substitution Γ (varFC m τ Δ) (snoc es e)
+    | TypedLockCtxt : forall (Γ : Ctxt) (Δ : FiniteCtxt) (m : mod) (es : list expr),
+        typed_finite_substitution (add_lock Γ m) Δ es ->
+        typed_finite_substitution Γ (lockFC m Δ) es.
+
+    Lemma typed_finite_substitution_length : forall Γ Δ es,
+        typed_finite_substitution Γ Δ es ->
+        FiniteCtxtSize Δ = length es.
+    Proof using.
+      intros Γ Δ es typd; induction typd; cbn; try rewrite snoc_length; auto.
+    Qed.
+
+    Lemma finite_substitution_past_length : forall es n,
+        length es <= n ->
+        finite_substitution es n = var (n - length es).
+    Proof using.
+      intro es; induction es; destruct n; cbn; intro length_le_n; auto.
+      inversion length_le_n.
+      rewrite IHes; [reflexivity|].
+      apply le_S_n; exact length_le_n.
+    Qed.
+
+    Lemma finite_substitution_snoc_end : forall es e,
+        finite_substitution (snoc es e) (length es) = e.
+    Proof using.
+      intro es; induction es as [| e' es IHes]; intro e; cbn; [| rewrite IHes]; auto.
+    Qed.
+
+    Lemma finite_substitution_snoc_lt : forall es e n,
+        n < length es ->
+        finite_substitution (snoc es e) n = finite_substitution es n.
+    Proof using.
+      intro es; induction es as [| e' es IHes]; intros e n n_lt_len; cbn in *.
+      - inversion n_lt_len.
+      - destruct n; [reflexivity|].
+        apply IHes.
+        apply PeanoNat.lt_S_n; exact n_lt_len.
+    Qed.
+
+    Lemma typed_finite_subst_typed : forall Γ Δ es n m m' τ,
+        typed_finite_substitution Γ Δ es ->
+        nth_var Δ n = Some (m, τ) ->
+        locks_at Δ n = Some m' ->
+        Typed (add_lock (add_lock Γ m') m) (finite_substitution es n) τ.
+    Proof using.
+      intros Γ Δ es n m m' τ typd; revert n m m' τ; induction typd; intros n m' m'' τ' eq1 eq2; cbn in *.
+      - unfold nth_var in eq1; destruct n; cbn in eq1; inversion eq1.
+      - unfold nth_var in eq1; cbn in eq1; unfold locks_at in eq2; cbn in eq2.
+        destruct (Compare_dec.le_lt_dec (FiniteCtxtSize Δ) n) as [size_le_n | n_lt_size].
+        -- destruct (Compare_dec.le_lt_eq_dec _ _ size_le_n) as [size_lt_n | size_eq_n].
+           --- rewrite List.nth_error_app2 in eq1; [| rewrite <- vars_of_finite_ctxt_size; auto].
+               rewrite List.nth_error_app2 in eq2; [| rewrite locks_at_finite_ctxt_vars_size; auto].
+               rewrite <- vars_of_finite_ctxt_size in eq1; rewrite locks_at_finite_ctxt_vars_size in eq2.
+               destruct (n - FiniteCtxtSize Δ) as [| n'] eqn:eq; cbn in eq1; cbn in eq2.
+               exfalso; lia.
+               rewrite List.nth_error_nil in eq1; inversion eq1.
+           --- rewrite List.nth_error_app2 in eq1; [| rewrite <- vars_of_finite_ctxt_size; auto].
+               rewrite List.nth_error_app2 in eq2; [| rewrite locks_at_finite_ctxt_vars_size; auto].
+               rewrite <- vars_of_finite_ctxt_size in eq1; rewrite locks_at_finite_ctxt_vars_size in eq2.
+               rewrite size_eq_n in eq1; rewrite PeanoNat.Nat.sub_diag in eq1;
+                 rewrite size_eq_n in eq2; rewrite PeanoNat.Nat.sub_diag in eq2; cbn in eq1; cbn in eq2.
+               inversion eq1; subst; clear eq1; inversion eq2; subst.
+               pose proof (typed_finite_substitution_length _ _ _ typd).
+               rewrite H1 at 1. rewrite finite_substitution_snoc_end; auto.
+        -- rewrite List.nth_error_app1 in eq1; [| rewrite <- vars_of_finite_ctxt_size; auto].
+           rewrite List.nth_error_app1 in eq2; [| rewrite locks_at_finite_ctxt_vars_size; auto].
+           rewrite finite_substitution_snoc_lt. 2: rewrite <- (typed_finite_substitution_length _ _ _ typd); auto.
+           apply IHtypd; auto.
+      - unfold locks_at in eq2; cbn in eq2.
+        unfold nth_var in eq1; cbn in eq1.
+        admit.
+    Abort.
+           
+
+    Theorem finite_subst_typed : forall Γ e Δ E es τ,
+        Typed (addFiniteCtxt (addFiniteCtxt Γ Δ) E) e τ ->
+        typed_finite_substitution Γ Δ es ->
+        Typed (addFiniteCtxt (add_lock Γ (FiniteCtxtLocks Δ)) E) (subst e (substup_many (FiniteCtxtSize E) (finite_substitution es))) τ.
+    Proof using.
+      intros Γ e; revert Γ; induction e; intros Γ Δ E es τ typd typd_subst; cbn; inversion typd; subst; 
+        try (econstructor; eauto; fail).
+      - destruct (Compare_dec.le_lt_dec (FiniteCtxtSize E) n).
+        -- rewrite vars_past_finite_ctxt in pf1; auto.
+           rewrite AddFiniteCtxt_locks1 in pf1; auto.
+           unfold substup_many. rewrite (proj2 (PeanoNat.Nat.ltb_ge _ _) l).
+           destruct (Compare_dec.le_lt_dec (FiniteCtxtSize Δ) (n - FiniteCtxtSize E)) as [l' | l'].
+           ---
+             eapply weakening. apply extend_rename.
+             rewrite finite_substitution_past_length; [|rewrite <- (typed_finite_substitution_length _ _ _ typd_subst); exact l'].
+               cbn. 
+               rewrite vars_past_finite_ctxt in pf1; auto.
+               rewrite AddFiniteCtxt_locks1 in pf1; auto.
+               rewrite <- (typed_finite_substitution_length _ _ _ typd_subst).
+               eapply VarTyping; cbn. exact pf1. reflexivity.
+           --- eapply weakening with (mono := add_mono (FiniteCtxtSize E)).
+               apply extend_rename.
+      (*          apply typed_finite_subst_typed with (Δ := Δ); auto. *)
+      (*          rewrite vars_in_finite_ctxt with (Γ:= Γ); auto. *)
+      (*          rewrite pf1; f_equal. *)
+      (*          pose proof (AddFiniteCtxt_locks2 Γ Δ (n - FiniteCtxtSize E) l') *)
+      (*      admit. *)
+      (*   -- unfold substup_many; rewrite (proj2 (PeanoNat.Nat.ltb_lt n (FiniteCtxtSize E))); [| exact l]. *)
+      (*        apply @VarTyping with (m := locks (addFiniteCtxt Γ E) n). *)
+      (*        2: { pose proof (AddFiniteCtxt_locks2 (add_lock Γ (FiniteCtxtLocks Δ)) E n l). *)
+      (*             pose proof (AddFiniteCtxt_locks2 Γ E n l). *)
+      (*             rewrite <- H1 in H0; inversion H0; reflexivity. } *)
+      (*        destruct (nth_var_size1 E n l) as [m [τ' eq]]. *)
+      (*        assert (vars (addFiniteCtxt (addFiniteCtxt Γ Δ) E) n = (m, τ')) as eq' *)
+      (*            by (apply nth_var_add_ctxt; auto). *)
+      (*        rewrite nth_var_add_ctxt with (pr := (m, τ')); auto. *)
+      (*        rewrite eq' in pf1; inversion pf1; subst; clear pf1. *)
+      (*        f_equal. *)
+      (*        pose proof (AddFiniteCtxt_locks2 Γ E n l). *)
+      (*        pose proof (AddFiniteCtxt_locks2 (addFiniteCtxt Γ Δ) E n l). *)
+      (*        rewrite <- H1 in H0; inversion H0; subst; reflexivity. *)
+      (* - *)
+        
+             
+      (*   unfold substup_many. *)
+      (*   assert (PeanoNat.Nat.ltb n (FiniteCtxtSize E) = false) as eq by (rewrite PeanoNat.Nat.ltb_ge; auto); rewrite eq. *)
+        
+
+      (*   destruct (Compare_dec.le_lt_dec (FiniteCtxtSize Δ) n). *)
+      (*   rewrite finite_substitution_past_length. *)
+      (*   apply @VarTyping with (m := locks (addFiniteCtxt Γ Δ) n). *)
+      (*   rewrite <- typed_finite_substitution_length with (Γ := Γ) (Δ := Δ); auto. *)
+      (*   rewrite <- vars_past_finite_ctxt; auto. *)
+      (*   admit. *)
+      (*   erewrite <- typed_finite_substitution_length; eauto. *)
+      (*   admit. *)
+      (* -  eapply AtTyping. apply IHe with (xs := xs). *)
+      (*    admit. *)
+      (*    admit. *)
+      (* - apply @LetTyping with (τ := τ0). *)
+      (*   apply IHe1 with (xs := xs); auto. *)
+      (*   pose proof (IHe2 Γ (List.cons (proc_to_mod p, τ0) xs) (List.cons (var 0) es) τ). *)
+        
+               (*   apply IHe2 with (xs := (List.cons (proc_to_mod p, τ0) xs)). *)
+    Abort.
+      
+
+(*     Definition TypedSubst (Γ : Ctxt) (σ : substitution) (ξ : renaming) (Δ : Ctxt) := *)
+(*       all_locks Γ = all_locks Δ /\ *)
+(*         (forall n, PrefixOf (locks Γ n) (locks Δ (ξ n))) /\  *)
+(*         (* forall x m, *) *)
+(*         (*   mod_app m (locks Γ x) = fst (vars Γ x) ->  *) *)
+(*         (*   Typed (add_lock Δ m) (renseen (σ x) ξ) (snd (vars Γ x)). *) *)
+(*         (forall x, Typed (add_lock (remove_locks Δ) (owner_unqualified Γ x)) (renseen (σ x) ξ) (snd (vars Γ x))). *)
+
+(*     Lemma TypedSubst_ext  : forall (Γ1 Γ2 : Ctxt) (σ1 σ2 : substitution) (ξ1 ξ2 : renaming) (Δ1 Δ2 : Ctxt), *)
+(*         ctxt_equiv Γ1 Γ2 -> *)
+(*         (forall n, σ1 n = σ2 n) -> *)
+(*         (forall n, ξ1 n = ξ2 n) -> *)
+(*         ctxt_equiv Δ1 Δ2 -> *)
+(*         TypedSubst Γ1 σ1 ξ1 Δ1 -> *)
+(*         TypedSubst Γ2 σ2 ξ2 Δ2. *)
+(*     Proof using. *)
+(*       intros Γ1 Γ2 σ1 σ2 ξ1 ξ2 Δ1 Δ2 Γ_eqv σ_eqv ξ_eqv Δ_eqv [al_eqv3 [pfx typd]]; split; [|split]; *)
+(*         pose proof Γ_eqv as [vars_eqv1 [locks_eqv1 al_eqv1]]; *)
+(*         pose proof Δ_eqv as [vars_eqv2 [locks_eqv2 al_eqv2]]. *)
+(*       - rewrite <- al_eqv1; rewrite <- al_eqv2; exact al_eqv3. *)
+(*       - intro n; rewrite <- locks_eqv1; rewrite <- locks_eqv2; rewrite <- ξ_eqv; apply pfx. *)
+(*       - intros x. apply @type_ext with (Γ := add_lock (remove_locks Δ1) (owner_unqualified Γ1 x)); auto. *)
+(*         rewrite <- σ_eqv. rewrite <- renseen_ext with (ξ1 := ξ1); auto. *)
+(*         rewrite <- vars_eqv1. apply typd. *)
+(*         admit. *)
+(* Admitted. *)
+
+(*     Lemma id_subst_typed: forall Γ, TypedSubst Γ (fun x => var x) (fun x => x) Γ. *)
+(*     Proof using. *)
+(*       intros Γ; split; [reflexivity |  split; [reflexivity| intro x; cbn]]. *)
+(*       apply VarTyping with (m := owner_unqualified Γ x); cbn; auto. *)
+(*     Qed.       *)
+
+(*     Lemma substup_typed : forall Γ Δ σ ξ g τ, *)
+(*         TypedSubst Γ σ ξ Δ -> TypedSubst (add_var Γ g τ) (substup σ) (renup ξ) (add_var Δ g τ). *)
+(*     Proof using. *)
+(*       intros Γ Δ σ ξ g τ [al_eqv [pfx typd]]; split; [exact al_eqv|split]; [|intros x]. *)
+(*       - intro n; destruct n; cbn; [reflexivity | auto]. *)
+(*       - destruct x; cbn in *; subst. *)
+(*         -- admit. *)
+(*         -- rewrite renseen_fusion. *)
+(*            rewrite ren_renseen. cbn. rewrite <- renseen_fusion. rewrite <- ren_renseen. *)
+(*            eapply weakening; [| apply typd; apply eq]. *)
+(*            split; [|split]; try (intro y); cbn; auto. *)
+(*            Unshelve. 4: apply le_n_S. *)
+(*     Admitted. *)
+
+(*     Lemma addlock_typedsubst : forall Γ Δ σ ξ m, *)
+(*         TypedSubst Γ σ ξ Δ -> TypedSubst (add_lock Γ m) σ ξ (add_lock Δ m). *)
+(*     Proof using. *)
+(*       intros Γ Δ σ ξ m [al [pfx typd]]; split; [| split]; cbn; auto. *)
+(*       - rewrite al; reflexivity. *)
+(*       - intro n; apply mod_app_mono_l; apply pfx. *)
+(*       - intros x. *)
+(*         admit. *)
+(*     Admitted. *)
+
+(*     (* Lemma changelock_typedsubst : forall Γ Δ σ ξ {m1 m2} (inv1 : forall n, PrefixOf m1 (locks Γ n) \/ PrefixOf (locks Γ n) m2) *) *)
+(*     (*                                 (inv2 : forall n, PrefixOf m1 (locks Δ n) \/ PrefixOf (locks Δ n) m2), *) *)
+(*     (*     TypedSubst Γ σ ξ Δ -> *) *)
+(*     (*     TypedSubst (change_lock Γ inv1) σ ξ (change_lock Δ inv2). *) *)
+(*     (* Proof using. *) *)
+(*     (*   intros Γ Δ σ ξ m1 m2 inv1 inv2 [al_eqv [pfx typd]]; split; [| split]. *) *)
+(*     (*   - cbn; rewrite al_eqv; reflexivity. *) *)
+(*     (*   - intro n; cbn. admit. *) *)
+(*     (*   - intros x m eq. *) *)
+(*     (*     cbn. apply typd. *) *)
+
+      
+
+        
+
+(*     Theorem subst_typed : forall Γ Δ e σ ξ τ, Typed Γ e τ -> TypedSubst Γ σ ξ Δ -> Typed Δ (renseen (subst e σ) ξ) τ. *)
+(*     Proof using. *)
+(*       intros Γ Δ e σ ξ τ typed; revert Δ σ ξ; induction typed; try (rename σ into τ'); *)
+(*         intros Γ'' σ ξ typeds; cbn; pose proof typeds as [al_eqv [pfx typd]]. *)
+(*       all: try (econstructor; eauto; fail). *)
+(*       - *)
+        
+(*       (* assert (snd (vars Γ n) = τ) as x_tau by (rewrite pf1; reflexivity); rewrite <- x_tau. *) *)
+(*         (* apply @type_ext with (Γ := add_lock Γ'' base); [|symmetry; apply add_base_lock]. *) *)
+(*         (* apply typd. rewrite pf2. rewrite mod_base_app; auto. rewrite pf1; reflexivity. *) *)
+(*       - apply AtTyping. apply IHtyped. *)
+(*         apply addlock_typedsubst; auto. *)
+(*       - eapply LetTyping. apply IHtyped1; auto. *)
+(*         apply IHtyped2; apply substup_typed;auto. *)
+(*       - eapply CaseTyping. apply IHtyped1; auto. apply IHtyped2. 2: apply IHtyped3. all: apply substup_typed; auto. *)
+(*       - apply LamTyping. apply IHtyped. apply substup_typed. auto. *)
+(*       - eapply @SendTyping. reflexivity. *)
+(*         apply IHtyped. *)
+    (*     Qed.                                              *)
+
+
+    Definition single_subst (e : expr) : substitution :=
+      fun n =>
+        match n with
+        | 0 => e
+        | S n => var n
+        end.
+
+    
+    Theorem finite_subst_typed : forall (Γ : Ctxt) (Δ: FiniteCtxt) (e e' : expr) (m : mod) (τ τ' : type),
+        Typed (addFiniteCtxt (add_var Γ m τ') Δ) e τ ->
+        Typed (add_lock Γ m) e' τ' ->
+        Typed (addFiniteCtxt Γ Δ) (subst e (substup_many (FiniteCtxtSize Δ) (single_subst e'))) τ.
+    Proof using.
+      intros Γ Δ e; revert Γ Δ; induction e; intros Γ Δ e'' m' τ τ' typd1 typd2;
+        inversion typd1; subst; cbn; try (econstructor; eauto; fail).
+      - destruct (Compare_dec.le_lt_dec (FiniteCtxtSize Δ) n) as [ size_Δ_le_n | n_lt_size_Δ].
+        -- unfold substup_many. rewrite (proj2 (PeanoNat.Nat.ltb_ge _ _)); [| lia].
+           rewrite vars_past_finite_ctxt in pf1; [| lia].
+           rewrite AddFiniteCtxt_locks1 in pf1; [| lia].
+           destruct (n - FiniteCtxtSize Δ) eqn:eq; cbn.
+           --- eapply weakening. apply extend_rename.
+               cbn in pf1. inversion pf1; subst; auto.
+           --- assert (n0 + FiniteCtxtSize Δ - FiniteCtxtSize Δ = n0) as eq' by lia.
+               eapply VarTyping.
+               rewrite vars_past_finite_ctxt; [| lia]. rewrite eq'; exact pf1.
+               rewrite AddFiniteCtxt_locks1; [| lia]. rewrite eq'. reflexivity.
+        -- unfold substup_many. rewrite (proj2 (PeanoNat.Nat.ltb_lt _ _)); [| exact n_lt_size_Δ].
+           pose proof (vars_in_finite_ctxt Γ Δ n n_lt_size_Δ) as eq1.
+           pose proof (vars_in_finite_ctxt (add_var Γ m' τ') Δ n n_lt_size_Δ) as eq2.
+           eapply VarTyping.
+           rewrite eq1 in eq2; inversion eq2; subst. rewrite H1. rewrite pf1; reflexivity.
+           pose proof (AddFiniteCtxt_locks2 Γ Δ n n_lt_size_Δ) as eq3.
+           pose proof (AddFiniteCtxt_locks2 (add_var Γ m' τ') Δ n n_lt_size_Δ) as eq4.
+           rewrite <- eq3 in eq4; inversion eq4; subst.
+           reflexivity.
+      - apply AtTyping.
+        apply @type_ext with (Γ := addFiniteCtxt Γ (add_end_lock Δ p)); [| apply add_end_lock_eqv].
+        rewrite <- add_end_lock_size with (m := p).
+        apply IHe with (m := m') (τ' := τ'); auto.
+        eapply type_ext; eauto. symmetry; apply add_end_lock_eqv.
+      - apply @LetTyping with (τ := τ0).
+        -- apply IHe1 with (m := m') (τ' := τ'); auto.
+        -- eapply type_ext; [| apply add_end_var_eqv].
+           rewrite subst_ext with (σ2 := substup_many (FiniteCtxtSize (add_end_var Δ p τ0)) (single_subst e'')).
+           2: intro n; rewrite add_end_var_size; symmetry; apply substup_many_S.
+           apply IHe2 with (m := m') (τ' := τ'); auto.
+           eapply type_ext; [| symmetry; apply add_end_var_eqv]; auto.
+      - apply @CaseTyping with (τ1 := τ1) (τ2 := τ2).
+        -- apply IHe1 with (m := m') (τ' := τ'); auto.
+        -- eapply type_ext; [| apply add_end_var_eqv].
+           rewrite subst_ext with (σ2 := substup_many (FiniteCtxtSize (add_end_var Δ base τ1)) (single_subst e'')).
+           2: intro n; rewrite add_end_var_size; symmetry; apply substup_many_S.
+           apply IHe2 with (m := m') (τ' := τ'); auto.
+           eapply type_ext; [| symmetry; apply add_end_var_eqv]; auto.
+        -- eapply type_ext; [| apply add_end_var_eqv].
+           rewrite subst_ext with (σ2 := substup_many (FiniteCtxtSize (add_end_var Δ base τ2)) (single_subst e'')).
+           2: intro n; rewrite add_end_var_size; symmetry; apply substup_many_S.
+           apply IHe3 with (m := m') (τ' := τ'); auto.
+           eapply type_ext; [| symmetry; apply add_end_var_eqv]; auto.
+      - apply @LamTyping with (τ1 := t).  
+        eapply type_ext; [| apply add_end_var_eqv].
+        rewrite subst_ext with (σ2 := substup_many (FiniteCtxtSize (add_end_var Δ base t)) (single_subst e'')).
+        2: intro n; rewrite add_end_var_size; symmetry; apply substup_many_S.
+        apply IHe with (m := m') (τ' := τ'); auto.
+        eapply type_ext; [| symmetry; apply add_end_var_eqv]; auto.
+      - unshelve (eapply @SendTyping; [reflexivity | | auto]).
+        -- destruct (Compare_dec.le_gt_dec (FiniteCtxtSize Δ) seen).
+           --- assert (locks (addFiniteCtxt Γ Δ) seen = locks (addFiniteCtxt (add_var Γ m' τ') Δ) (1 + seen)).
+               repeat rewrite AddFiniteCtxt_locks1; try lia; apply f_equal.
+               assert (1 + seen - FiniteCtxtSize Δ = S (seen - FiniteCtxtSize Δ)) by lia.
+               rewrite H0; cbn; reflexivity.
+               rewrite H0; transitivity (locks (addFiniteCtxt (add_var Γ m' τ') Δ) seen); auto.
+               apply locks_mono; lia.
+           --- assert (Some (locks (addFiniteCtxt Γ Δ) seen) = Some (locks (addFiniteCtxt (add_var Γ m' τ') Δ) seen))
+                 by (repeat rewrite AddFiniteCtxt_locks2; auto).
+               inversion H0; rewrite H2; exact locks_seen.
+        -- 
+      - unshelve (eapply @UpTyping; eauto).
+
+        
   End Substitution.
   
 End CorpsTypes.
